Veir/Rewriter/WellFormed/EraseOp.lean
@@ -1,0 +1,1798 @@
+module
+
+public import Veir.Rewriter.Basic
+public import Veir.Rewriter.LinkedList.WellFormed
+public import Veir.IR.DeallocLemmas
+
+public section
+
+namespace Veir
+
+set_option maxHeartbeats 400000
+set_option maxRecDepth 8000
+
+variable {OpInfo : Type} [HasOpInfo OpInfo] [SerializableOpInfo OpInfo] [HasBuffedOpCode OpInfo]
+
+@[grind =]
+theorem Rewriter.detachOp_veir_inBounds
+    (ctx : Sim.IRContext OpInfo) (op : Sim.OperationPtr)
+    (hctx : ctx.spec.FieldsInBounds) (hIn : op.InBounds ctx)
+    (hasParent : (op.getParent ctx hIn).toOption.isSome)
+    (ptr : Veir.GenericPtr) :
+    ptr.InBounds (Rewriter.detachOp ctx op hctx hIn hasParent).spec ↔
+      ptr.InBounds ctx.spec := by
+  simp only [Rewriter.detachOp_def, Rewriter.detachOpSim,
+    Rewriter.unsetParentAndNeighbors_def, Rewriter.unsetParentAndNeighborsSim]
+  split <;> split <;> grind
+
+@[simp]
+theorem BlockPtr.firstUse!_detachOp
+    (ctx : Sim.IRContext OpInfo) (op : Sim.OperationPtr)
+    (hctx : ctx.spec.FieldsInBounds) (hIn : op.InBounds ctx)
+    (hasParent : (op.getParent ctx hIn).toOption.isSome)
+    (block : Veir.BlockPtr) :
+    (block.get! (Rewriter.detachOp ctx op hctx hIn hasParent).spec).firstUse =
+      (block.get! ctx.spec).firstUse := by
+  simp only [Rewriter.detachOp_def, Rewriter.detachOpSim,
+    Rewriter.unsetParentAndNeighbors_def, Rewriter.unsetParentAndNeighborsSim]
+  split <;> split
+  all_goals
+    simp only [Sim.BlockPtr.setFirstOp_spec, Sim.BlockPtr.setLastOp_spec,
+      Sim.OperationPtr.setNextOp_spec, Sim.OperationPtr.setPrevOp_spec,
+      Sim.OperationPtr.setParent_spec,
+      BlockPtr.firstUse!_BlockPtr_setFirstOp, BlockPtr.firstUse!_BlockPtr_setLastOp,
+      BlockPtr.get!_OperationPtr_setNextOp, BlockPtr.get!_OperationPtr_setPrevOp,
+      BlockPtr.get!_OperationPtr_setParent]
+
+@[simp]
+theorem OperationPtr.parent!_detachOp
+    (ctx : Sim.IRContext OpInfo) (op : Sim.OperationPtr)
+    (hctx : ctx.spec.FieldsInBounds) (hIn : op.InBounds ctx)
+    (hasParent : (op.getParent ctx hIn).toOption.isSome)
+    (operation : Veir.OperationPtr) :
+    (operation.get! (Rewriter.detachOp ctx op hctx hIn hasParent).spec).parent =
+      if operation = op.spec then none else (operation.get! ctx.spec).parent := by
+  simp only [Rewriter.detachOp_def, Rewriter.detachOpSim,
+    Rewriter.unsetParentAndNeighbors_def, Rewriter.unsetParentAndNeighborsSim]
+  split <;> split
+  all_goals
+    simp only [Sim.BlockPtr.setFirstOp_spec, Sim.BlockPtr.setLastOp_spec,
+      Sim.OperationPtr.setNextOp_spec, Sim.OperationPtr.setPrevOp_spec,
+      Sim.OperationPtr.setParent_spec,
+      OperationPtr.get!_BlockPtr_setFirstOp, OperationPtr.get!_BlockPtr_setLastOp,
+      OperationPtr.parent!_OperationPtr_setNextOp,
+      OperationPtr.parent!_OperationPtr_setPrevOp,
+      OperationPtr.parent!_OperationPtr_setParent]
+    split <;> rfl
+
+theorem BlockPtr.firstOp!_detachOp
+    (ctx : Sim.IRContext OpInfo) (op : Sim.OperationPtr)
+    (hctx : ctx.spec.FieldsInBounds) (hIn : op.InBounds ctx)
+    (hasParent : (op.getParent ctx hIn).toOption.isSome)
+    (block : Veir.BlockPtr) :
+    (block.get! (Rewriter.detachOp ctx op hctx hIn hasParent).spec).firstOp =
+      if (op.spec.get! ctx.spec).prev = none ∧
+          some block = (op.spec.get! ctx.spec).parent then
+        (op.spec.get! ctx.spec).next
+      else (block.get! ctx.spec).firstOp := by
+  have hPrevIB : (op.getPrevOp ctx hIn).InBounds ctx := by grind
+  have hParentIB : (op.getParent ctx hIn).InBounds ctx := by grind
+  have hPrevNone : (op.getPrevOp ctx hIn).toOption = none ↔
+      (op.spec.get! ctx.spec).prev = none := by
+    rw [Sim.OptionOperationPtr.toOption_none_iff_spec_none hPrevIB,
+      Sim.OperationPtr.getPrevOp_spec ctx op hIn]
+    rw [OperationPtr.get!_eq_get]
+  have hNextSpec := Sim.OperationPtr.getNextOp_spec ctx op hIn
+  have hNextSpecBang : (op.getNextOp ctx hIn).spec =
+      (op.spec.get! ctx.spec).next := by
+    rw [OperationPtr.get!_eq_get]
+    exact hNextSpec
+  have hParentSome : (op.getParent ctx hIn).spec =
+      some ((op.getParent ctx hIn).toOption.get hasParent).spec := by
+    apply Sim.OptionBlockPtr.toOption_some hParentIB
+    exact (Option.some_get hasParent).symm
+  rw [Sim.OperationPtr.getParent_spec ctx op hIn] at hParentSome
+  have hParentSomeBang : (op.spec.get! ctx.spec).parent =
+      some ((op.getParent ctx hIn).toOption.get hasParent).spec := by
+    rw [OperationPtr.get!_eq_get]
+    exact hParentSome
+  simp only [Rewriter.detachOp_def, Rewriter.detachOpSim,
+    Rewriter.unsetParentAndNeighbors_def, Rewriter.unsetParentAndNeighborsSim]
+  split
+  next prev hprev =>
+    have hp : (op.spec.get! ctx.spec).prev ≠ none := by
+      intro hp
+      have hnone := hPrevNone.mpr hp
+      simpa [hprev] using hnone
+    split <;>
+    simp only [Sim.BlockPtr.setFirstOp_spec, Sim.BlockPtr.setLastOp_spec,
+      Sim.OperationPtr.setNextOp_spec, Sim.OperationPtr.setPrevOp_spec,
+      Sim.OperationPtr.setParent_spec,
+      BlockPtr.firstOp!_BlockPtr_setFirstOp, BlockPtr.firstOp!_BlockPtr_setLastOp,
+      BlockPtr.get!_OperationPtr_setNextOp, BlockPtr.get!_OperationPtr_setPrevOp,
+      BlockPtr.get!_OperationPtr_setParent]
+    all_goals rw [if_neg (fun h => hp h.1)]
+  next hprev =>
+    have hp : (op.spec.get! ctx.spec).prev = none := hPrevNone.mp hprev
+    split <;>
+      simp only [Sim.BlockPtr.setFirstOp_spec, Sim.BlockPtr.setLastOp_spec,
+        Sim.OperationPtr.setNextOp_spec, Sim.OperationPtr.setPrevOp_spec,
+        Sim.OperationPtr.setParent_spec,
+        BlockPtr.firstOp!_BlockPtr_setFirstOp, BlockPtr.firstOp!_BlockPtr_setLastOp,
+        BlockPtr.get!_OperationPtr_setNextOp, BlockPtr.get!_OperationPtr_setPrevOp,
+        BlockPtr.get!_OperationPtr_setParent]
+    all_goals
+      by_cases hb : some block = (op.spec.get! ctx.spec).parent
+      · simp only [hp, true_and]
+        rw [if_pos hb]
+        have hpb : ((op.getParent ctx hIn).toOption.get hasParent).spec = block := by
+          rw [hParentSomeBang] at hb
+          exact Option.some.inj hb.symm
+        rw [if_pos hpb, hNextSpecBang]
+      · simp only [hp, true_and]
+        rw [if_neg hb]
+        have hpb : ((op.getParent ctx hIn).toOption.get hasParent).spec ≠ block := by
+          intro hpb
+          apply hb
+          rw [hParentSomeBang, hpb]
+        rw [if_neg hpb]
+
+theorem Rewriter.detachOperands.loop_wellFormed
+    (ctx : Sim.IRContext OpInfo) (op : Sim.OperationPtr) (off : Int64) (index : UInt64)
+    (hCtx : ctx.spec.FieldsInBounds) (hOp : op.InBounds ctx)
+    (hIndex : index.toNat < op.spec.getNumOperands! ctx.spec)
+    (hoff : off = Buffed.Operation.Offsets.operands op.spec ctx.spec)
+    (wf : ctx.spec.WellFormed missingOperands missingSuccessors)
+    (hMissing : ∀ i, i ≤ index.toNat → OpOperandPtr.mk op.spec i ∉ missingOperands) :
+    (Rewriter.detachOperands.loop ctx op off index hCtx hOp hIndex hoff).spec.WellFormed
+      (missingOperands.insertMany
+        ((0...=index.toNat).toList.map (fun i => OpOperandPtr.mk op.spec i)))
+      missingSuccessors := by
+  simp only [Rewriter.detachOperands.loop_def]
+  fun_induction Rewriter.detachOperands.loopSim generalizing missingOperands missingSuccessors
+  case case1 =>
+    let use := op.getOperandPtrAt _ off 0 (by assumption) (by assumption)
+    have hUseSpec : use.spec = OpOperandPtr.mk op.spec 0 := rfl
+    have hwf := Sim.IRContext.wellFormed_OpOperandPtr_removeFromCurrent
+      (use := use) (useInBounds := by
+        dsimp [use]
+        rw [Sim.OperationPtr.getOperandPtrAt_eq_getOperandPtr]
+        exact Sim.OperationPtr.getOpOperand_inBounds op (by assumption) 0 (by assumption))
+      (ctxInBounds := wf.inBounds)
+      (useMissing := by simpa [hUseSpec] using hMissing 0 (by simp)) wf
+    simpa [use, hUseSpec, Nat.toList_rcc_eq_singleton,
+      Std.ExtHashSet.insertMany_list_singleton] using hwf
+  case case2 =>
+    rename_i _ _ _ currentCtx currentIndex hCtxCur hOpCur hIndexCur hoffCur currentCtx' hne ih
+    have hCurrentPos : 0 < currentIndex.toNat := by
+      have hneNat : currentIndex.toNat ≠ 0 := by
+        intro hz
+        apply hne
+        apply UInt64.toNat_inj.mp
+        simpa using hz
+      omega
+    have hCurrentLt := UInt64.toNat_lt currentIndex
+    have hPred : (currentIndex - 1).toNat = currentIndex.toNat - 1 := by
+      rw [UInt64.toNat_sub]
+      change (2 ^ 64 - 1 + currentIndex.toNat) % 2 ^ 64 = currentIndex.toNat - 1
+      have heq : 2 ^ 64 - 1 + currentIndex.toNat =
+          2 ^ 64 + (currentIndex.toNat - 1) := by omega
+      rw [heq, Nat.add_mod]
+      simp only [Nat.mod_self, Nat.zero_add]
+      rw [Nat.mod_eq_of_lt (by omega), Nat.mod_eq_of_lt (by omega)]
+    let use := op.getOperandPtrAt currentCtx off currentIndex (by assumption) (by assumption)
+    have hUseSpec : use.spec = OpOperandPtr.mk op.spec currentIndex.toNat := rfl
+    have hwfRemoved := Sim.IRContext.wellFormed_OpOperandPtr_removeFromCurrent
+      (use := use) (useInBounds := by
+        dsimp [use]
+        rw [Sim.OperationPtr.getOperandPtrAt_eq_getOperandPtr]
+        exact Sim.OperationPtr.getOpOperand_inBounds op (by assumption) currentIndex (by assumption))
+      (ctxInBounds := wf.inBounds)
+      (useMissing := by
+        rw [hUseSpec]
+        exact hMissing currentIndex.toNat (Nat.le_refl _)) wf
+    have hwfRec := ih hwfRemoved (by
+      intro i hi
+      simp only [Std.ExtHashSet.mem_insert, hUseSpec, not_or]
+      constructor
+      · simp only [beq_iff_eq, OpOperandPtr.mk.injEq, true_and]
+        rw [hPred] at hi
+        omega
+      · apply hMissing i
+        rw [hPred] at hi
+        omega)
+    have hSets :
+        (missingOperands.insert use.spec).insertMany
+            ((0...=(currentIndex - 1).toNat).toList.map
+              (fun i => OpOperandPtr.mk op.spec i)) =
+          missingOperands.insertMany
+            ((0...=currentIndex.toNat).toList.map
+              (fun i => OpOperandPtr.mk op.spec i)) := by
+      rw [hUseSpec, Nat.toList_rcc_eq_toList_rco, hPred]
+      have hSucc : currentIndex.toNat - 1 + 1 = currentIndex.toNat := by omega
+      rw [hSucc, Nat.toList_rcc_eq_append (Nat.zero_le _), List.map_append,
+        List.map_singleton, Std.ExtHashSet.insertMany_append,
+        Std.ExtHashSet.insertMany_list_singleton,
+        Std.ExtHashSet.insertMany_list_insert_comm]
+    rw [hSets] at hwfRec
+    exact hwfRec
+
+theorem BlockPtr.lastOp!_detachOp
+    (ctx : Sim.IRContext OpInfo) (op : Sim.OperationPtr)
+    (hctx : ctx.spec.FieldsInBounds) (hIn : op.InBounds ctx)
+    (hasParent : (op.getParent ctx hIn).toOption.isSome)
+    (block : Veir.BlockPtr) :
+    (block.get! (Rewriter.detachOp ctx op hctx hIn hasParent).spec).lastOp =
+      if (op.spec.get! ctx.spec).next = none ∧
+          some block = (op.spec.get! ctx.spec).parent then
+        (op.spec.get! ctx.spec).prev
+      else (block.get! ctx.spec).lastOp := by
+  have hNextIB : (op.getNextOp ctx hIn).InBounds ctx := by grind
+  have hParentIB : (op.getParent ctx hIn).InBounds ctx := by grind
+  have hNextNone : (op.getNextOp ctx hIn).toOption = none ↔
+      (op.spec.get! ctx.spec).next = none := by
+    rw [Sim.OptionOperationPtr.toOption_none_iff_spec_none hNextIB,
+      Sim.OperationPtr.getNextOp_spec ctx op hIn]
+    rw [OperationPtr.get!_eq_get]
+  have hPrevSpec := Sim.OperationPtr.getPrevOp_spec ctx op hIn
+  have hPrevSpecBang : (op.getPrevOp ctx hIn).spec =
+      (op.spec.get! ctx.spec).prev := by
+    rw [OperationPtr.get!_eq_get]
+    exact hPrevSpec
+  have hParentSome : (op.getParent ctx hIn).spec =
+      some ((op.getParent ctx hIn).toOption.get hasParent).spec := by
+    apply Sim.OptionBlockPtr.toOption_some hParentIB
+    exact (Option.some_get hasParent).symm
+  rw [Sim.OperationPtr.getParent_spec ctx op hIn] at hParentSome
+  have hParentSomeBang : (op.spec.get! ctx.spec).parent =
+      some ((op.getParent ctx hIn).toOption.get hasParent).spec := by
+    rw [OperationPtr.get!_eq_get]
+    exact hParentSome
+  simp only [Rewriter.detachOp_def, Rewriter.detachOpSim,
+    Rewriter.unsetParentAndNeighbors_def, Rewriter.unsetParentAndNeighborsSim]
+  split
+  next prev hprev =>
+    split
+    next next hnext =>
+      have hn : (op.spec.get! ctx.spec).next ≠ none := by
+        intro hn
+        have := hNextNone.mpr hn
+        simp [hnext] at this
+      simp only [Sim.BlockPtr.setFirstOp_spec, Sim.BlockPtr.setLastOp_spec,
+        Sim.OperationPtr.setNextOp_spec, Sim.OperationPtr.setPrevOp_spec,
+        Sim.OperationPtr.setParent_spec,
+        BlockPtr.lastOp!_BlockPtr_setFirstOp, BlockPtr.lastOp!_BlockPtr_setLastOp,
+        BlockPtr.get!_OperationPtr_setNextOp, BlockPtr.get!_OperationPtr_setPrevOp,
+        BlockPtr.get!_OperationPtr_setParent]
+      rw [if_neg (fun h => hn h.1)]
+    next hnext =>
+      have hn : (op.spec.get! ctx.spec).next = none := hNextNone.mp hnext
+      simp only [Sim.BlockPtr.setFirstOp_spec, Sim.BlockPtr.setLastOp_spec,
+        Sim.OperationPtr.setNextOp_spec, Sim.OperationPtr.setPrevOp_spec,
+        Sim.OperationPtr.setParent_spec,
+        BlockPtr.lastOp!_BlockPtr_setFirstOp, BlockPtr.lastOp!_BlockPtr_setLastOp,
+        BlockPtr.get!_OperationPtr_setNextOp, BlockPtr.get!_OperationPtr_setPrevOp,
+        BlockPtr.get!_OperationPtr_setParent]
+      by_cases hb : some block = (op.spec.get! ctx.spec).parent
+      · simp only [hn, true_and]
+        rw [if_pos hb]
+        have hpb : ((op.getParent ctx hIn).toOption.get hasParent).spec = block := by
+          rw [hParentSomeBang] at hb
+          exact Option.some.inj hb.symm
+        rw [if_pos hpb]
+        have hp := Sim.OptionOperationPtr.toOption_some
+          (by grind : (op.getPrevOp ctx hIn).InBounds ctx) hprev
+        change some prev.spec = (op.spec.get! ctx.spec).prev
+        exact hp.symm.trans hPrevSpecBang
+      · simp only [hn, true_and]
+        rw [if_neg hb]
+        have hpb : ((op.getParent ctx hIn).toOption.get hasParent).spec ≠ block := by
+          intro hpb
+          apply hb
+          rw [hParentSomeBang, hpb]
+        rw [if_neg hpb]
+  next hprev =>
+    split
+    next next hnext =>
+      have hn : (op.spec.get! ctx.spec).next ≠ none := by
+        intro hn
+        have := hNextNone.mpr hn
+        simp [hnext] at this
+      simp only [Sim.BlockPtr.setFirstOp_spec, Sim.BlockPtr.setLastOp_spec,
+        Sim.OperationPtr.setNextOp_spec, Sim.OperationPtr.setPrevOp_spec,
+        Sim.OperationPtr.setParent_spec,
+        BlockPtr.lastOp!_BlockPtr_setFirstOp, BlockPtr.lastOp!_BlockPtr_setLastOp,
+        BlockPtr.get!_OperationPtr_setNextOp, BlockPtr.get!_OperationPtr_setPrevOp,
+        BlockPtr.get!_OperationPtr_setParent]
+      rw [if_neg (fun h => hn h.1)]
+    next hnext =>
+      have hn : (op.spec.get! ctx.spec).next = none := hNextNone.mp hnext
+      simp only [Sim.BlockPtr.setFirstOp_spec, Sim.BlockPtr.setLastOp_spec,
+        Sim.OperationPtr.setNextOp_spec, Sim.OperationPtr.setPrevOp_spec,
+        Sim.OperationPtr.setParent_spec,
+        BlockPtr.lastOp!_BlockPtr_setFirstOp, BlockPtr.lastOp!_BlockPtr_setLastOp,
+        BlockPtr.get!_OperationPtr_setNextOp, BlockPtr.get!_OperationPtr_setPrevOp,
+        BlockPtr.get!_OperationPtr_setParent]
+      by_cases hb : some block = (op.spec.get! ctx.spec).parent
+      · simp only [hn, true_and]
+        rw [if_pos hb]
+        have hpb : ((op.getParent ctx hIn).toOption.get hasParent).spec = block := by
+          rw [hParentSomeBang] at hb
+          exact Option.some.inj hb.symm
+        rw [if_pos hpb]
+        have hp := (Sim.OptionOperationPtr.toOption_none_iff_spec_none
+          (by grind : (op.getPrevOp ctx hIn).InBounds ctx)).mp hprev
+        simpa [hp] using hPrevSpecBang
+      · simp only [hn, true_and]
+        rw [if_neg hb]
+        have hpb : ((op.getParent ctx hIn).toOption.get hasParent).spec ≠ block := by
+          intro hpb
+          apply hb
+          rw [hParentSomeBang, hpb]
+        rw [if_neg hpb]
+
+theorem OperationPtr.prev!_detachOp
+    (ctx : Sim.IRContext OpInfo) (op : Sim.OperationPtr)
+    (hctx : ctx.spec.FieldsInBounds) (hIn : op.InBounds ctx)
+    (hasParent : (op.getParent ctx hIn).toOption.isSome)
+    (operation : Veir.OperationPtr) :
+    (operation.get! (Rewriter.detachOp ctx op hctx hIn hasParent).spec).prev =
+      if some operation = (op.spec.get! ctx.spec).next then
+        (op.spec.get! ctx.spec).prev
+      else if operation = op.spec then none else (operation.get! ctx.spec).prev := by
+  have hPrevIB : (op.getPrevOp ctx hIn).InBounds ctx := by grind
+  have hNextIB : (op.getNextOp ctx hIn).InBounds ctx := by grind
+  have hPrevSpec : (op.getPrevOp ctx hIn).spec =
+      (op.spec.get! ctx.spec).prev := by
+    rw [Sim.OperationPtr.getPrevOp_spec ctx op hIn, OperationPtr.get!_eq_get]
+  have hNextSpec : (op.getNextOp ctx hIn).spec =
+      (op.spec.get! ctx.spec).next := by
+    rw [Sim.OperationPtr.getNextOp_spec ctx op hIn, OperationPtr.get!_eq_get]
+  simp only [Rewriter.detachOp_def, Rewriter.detachOpSim,
+    Rewriter.unsetParentAndNeighbors_def, Rewriter.unsetParentAndNeighborsSim]
+  split <;> split
+  all_goals
+    simp only [Sim.BlockPtr.setFirstOp_spec, Sim.BlockPtr.setLastOp_spec,
+      Sim.OperationPtr.setNextOp_spec, Sim.OperationPtr.setPrevOp_spec,
+      Sim.OperationPtr.setParent_spec,
+      OperationPtr.get!_BlockPtr_setFirstOp, OperationPtr.get!_BlockPtr_setLastOp,
+      OperationPtr.prev!_OperationPtr_setNextOp,
+      OperationPtr.prev!_OperationPtr_setPrevOp,
+      OperationPtr.prev!_OperationPtr_setParent]
+  next prev hprev next hnext =>
+    have hp := Sim.OptionOperationPtr.toOption_some hPrevIB hprev
+    have hn := Sim.OptionOperationPtr.toOption_some hNextIB hnext
+    have hp' : (op.spec.get! ctx.spec).prev = some prev.spec := hPrevSpec.symm.trans hp
+    have hn' : (op.spec.get! ctx.spec).next = some next.spec := hNextSpec.symm.trans hn
+    have hnRaw := hn'
+    rw [OperationPtr.get!_eq_get (hin := hIn.ib)] at hnRaw
+    simp [hp', hn', hnRaw, Sim.OperationPtr.toO, Sim.OptionOperationPtr.none]
+  next prev hprev hnext =>
+    have hp := Sim.OptionOperationPtr.toOption_some hPrevIB hprev
+    have hn := (Sim.OptionOperationPtr.toOption_none_iff_spec_none hNextIB).mp hnext
+    have hp' : (op.spec.get! ctx.spec).prev = some prev.spec := hPrevSpec.symm.trans hp
+    have hn' : (op.spec.get! ctx.spec).next = none := hNextSpec.symm.trans hn
+    simp [hp', hn', Sim.OperationPtr.toO, Sim.OptionOperationPtr.none]
+  next hprev next hnext =>
+    have hp := (Sim.OptionOperationPtr.toOption_none_iff_spec_none hPrevIB).mp hprev
+    have hn := Sim.OptionOperationPtr.toOption_some hNextIB hnext
+    have hp' : (op.spec.get! ctx.spec).prev = none := hPrevSpec.symm.trans hp
+    have hn' : (op.spec.get! ctx.spec).next = some next.spec := hNextSpec.symm.trans hn
+    have hpRaw := hp'
+    rw [OperationPtr.get!_eq_get (hin := hIn.ib)] at hpRaw
+    simp [hp', hpRaw, hn', Sim.OperationPtr.toO, Sim.OptionOperationPtr.none]
+  next hprev hnext =>
+    have hp := (Sim.OptionOperationPtr.toOption_none_iff_spec_none hPrevIB).mp hprev
+    have hn := (Sim.OptionOperationPtr.toOption_none_iff_spec_none hNextIB).mp hnext
+    have hp' : (op.spec.get! ctx.spec).prev = none := hPrevSpec.symm.trans hp
+    have hn' : (op.spec.get! ctx.spec).next = none := hNextSpec.symm.trans hn
+    simp [hp', hn', Sim.OperationPtr.toO, Sim.OptionOperationPtr.none]
+
+theorem OperationPtr.next!_detachOp
+    (ctx : Sim.IRContext OpInfo) (op : Sim.OperationPtr)
+    (hctx : ctx.spec.FieldsInBounds) (hIn : op.InBounds ctx)
+    (hasParent : (op.getParent ctx hIn).toOption.isSome)
+    (operation : Veir.OperationPtr) :
+    (operation.get! (Rewriter.detachOp ctx op hctx hIn hasParent).spec).next =
+      if some operation = (op.spec.get! ctx.spec).prev then
+        (op.spec.get! ctx.spec).next
+      else if operation = op.spec then none else (operation.get! ctx.spec).next := by
+  have hPrevIB : (op.getPrevOp ctx hIn).InBounds ctx := by grind
+  have hNextIB : (op.getNextOp ctx hIn).InBounds ctx := by grind
+  have hPrevSpec : (op.getPrevOp ctx hIn).spec =
+      (op.spec.get! ctx.spec).prev := by
+    rw [Sim.OperationPtr.getPrevOp_spec ctx op hIn, OperationPtr.get!_eq_get]
+  have hNextSpec : (op.getNextOp ctx hIn).spec =
+      (op.spec.get! ctx.spec).next := by
+    rw [Sim.OperationPtr.getNextOp_spec ctx op hIn, OperationPtr.get!_eq_get]
+  simp only [Rewriter.detachOp_def, Rewriter.detachOpSim,
+    Rewriter.unsetParentAndNeighbors_def, Rewriter.unsetParentAndNeighborsSim]
+  split <;> split
+  all_goals
+    simp only [Sim.BlockPtr.setFirstOp_spec, Sim.BlockPtr.setLastOp_spec,
+      Sim.OperationPtr.setNextOp_spec, Sim.OperationPtr.setPrevOp_spec,
+      Sim.OperationPtr.setParent_spec,
+      OperationPtr.get!_BlockPtr_setFirstOp, OperationPtr.get!_BlockPtr_setLastOp,
+      OperationPtr.next!_OperationPtr_setNextOp,
+      OperationPtr.next!_OperationPtr_setPrevOp,
+      OperationPtr.next!_OperationPtr_setParent]
+  next prev hprev next hnext =>
+    have hp := Sim.OptionOperationPtr.toOption_some hPrevIB hprev
+    have hn := Sim.OptionOperationPtr.toOption_some hNextIB hnext
+    have hp' : (op.spec.get! ctx.spec).prev = some prev.spec := hPrevSpec.symm.trans hp
+    have hn' : (op.spec.get! ctx.spec).next = some next.spec := hNextSpec.symm.trans hn
+    have hnRaw := hn'
+    rw [OperationPtr.get!_eq_get (hin := hIn.ib)] at hnRaw
+    simp [hp', hn', hnRaw, Sim.OperationPtr.toO, Sim.OptionOperationPtr.none]
+  next prev hprev hnext =>
+    have hp := Sim.OptionOperationPtr.toOption_some hPrevIB hprev
+    have hn := (Sim.OptionOperationPtr.toOption_none_iff_spec_none hNextIB).mp hnext
+    have hp' : (op.spec.get! ctx.spec).prev = some prev.spec := hPrevSpec.symm.trans hp
+    have hn' : (op.spec.get! ctx.spec).next = none := hNextSpec.symm.trans hn
+    have hnRaw := hn'
+    rw [OperationPtr.get!_eq_get (hin := hIn.ib)] at hnRaw
+    simp [hp', hn', hnRaw, Sim.OperationPtr.toO, Sim.OptionOperationPtr.none]
+  next hprev next hnext =>
+    have hp := (Sim.OptionOperationPtr.toOption_none_iff_spec_none hPrevIB).mp hprev
+    have hn := Sim.OptionOperationPtr.toOption_some hNextIB hnext
+    have hp' : (op.spec.get! ctx.spec).prev = none := hPrevSpec.symm.trans hp
+    have hn' : (op.spec.get! ctx.spec).next = some next.spec := hNextSpec.symm.trans hn
+    simp [hp', hn', Sim.OperationPtr.toO, Sim.OptionOperationPtr.none]
+  next hprev hnext =>
+    have hp := (Sim.OptionOperationPtr.toOption_none_iff_spec_none hPrevIB).mp hprev
+    have hn := (Sim.OptionOperationPtr.toOption_none_iff_spec_none hNextIB).mp hnext
+    have hp' : (op.spec.get! ctx.spec).prev = none := hPrevSpec.symm.trans hp
+    have hn' : (op.spec.get! ctx.spec).next = none := hNextSpec.symm.trans hn
+    simp [hp', hn', Sim.OperationPtr.toO, Sim.OptionOperationPtr.none]
+
+@[simp]
+theorem OpOperandPtr.get!_detachOp
+    (ctx : Sim.IRContext OpInfo) (op : Sim.OperationPtr)
+    (hctx : ctx.spec.FieldsInBounds) (hIn : op.InBounds ctx)
+    (hasParent : (op.getParent ctx hIn).toOption.isSome)
+    (operand : Veir.OpOperandPtr) :
+    operand.get! (Rewriter.detachOp ctx op hctx hIn hasParent).spec =
+      operand.get! ctx.spec := by
+  simp only [Rewriter.detachOp_def, Rewriter.detachOpSim,
+    Rewriter.unsetParentAndNeighbors_def, Rewriter.unsetParentAndNeighborsSim]
+  split <;> split
+  all_goals simp only [Sim.BlockPtr.setFirstOp_spec, Sim.BlockPtr.setLastOp_spec,
+    Sim.OperationPtr.setNextOp_spec, Sim.OperationPtr.setPrevOp_spec,
+    Sim.OperationPtr.setParent_spec,
+    OpOperandPtr.get!_BlockPtr_setFirstOp, OpOperandPtr.get!_BlockPtr_setLastOp,
+    OpOperandPtr.get!_OperationPtr_setNextOp, OpOperandPtr.get!_OperationPtr_setPrevOp,
+    OpOperandPtr.get!_OperationPtr_setParent]
+
+@[simp]
+theorem BlockOperandPtr.get!_detachOp
+    (ctx : Sim.IRContext OpInfo) (op : Sim.OperationPtr)
+    (hctx : ctx.spec.FieldsInBounds) (hIn : op.InBounds ctx)
+    (hasParent : (op.getParent ctx hIn).toOption.isSome)
+    (operand : Veir.BlockOperandPtr) :
+    operand.get! (Rewriter.detachOp ctx op hctx hIn hasParent).spec =
+      operand.get! ctx.spec := by
+  simp only [Rewriter.detachOp_def, Rewriter.detachOpSim,
+    Rewriter.unsetParentAndNeighbors_def, Rewriter.unsetParentAndNeighborsSim]
+  split <;> split
+  all_goals simp only [Sim.BlockPtr.setFirstOp_spec, Sim.BlockPtr.setLastOp_spec,
+    Sim.OperationPtr.setNextOp_spec, Sim.OperationPtr.setPrevOp_spec,
+    Sim.OperationPtr.setParent_spec,
+    BlockOperandPtr.get!_BlockPtr_setFirstOp, BlockOperandPtr.get!_BlockPtr_setLastOp,
+    BlockOperandPtr.get!_OperationPtr_setNextOp, BlockOperandPtr.get!_OperationPtr_setPrevOp,
+    BlockOperandPtr.get!_OperationPtr_setParent]
+
+@[simp]
+theorem OpResultPtr.get!_detachOp
+    (ctx : Sim.IRContext OpInfo) (op : Sim.OperationPtr)
+    (hctx : ctx.spec.FieldsInBounds) (hIn : op.InBounds ctx)
+    (hasParent : (op.getParent ctx hIn).toOption.isSome)
+    (result : Veir.OpResultPtr) :
+    result.get! (Rewriter.detachOp ctx op hctx hIn hasParent).spec =
+      result.get! ctx.spec := by
+  simp only [Rewriter.detachOp_def, Rewriter.detachOpSim,
+    Rewriter.unsetParentAndNeighbors_def, Rewriter.unsetParentAndNeighborsSim]
+  split <;> split
+  all_goals simp only [Sim.BlockPtr.setFirstOp_spec, Sim.BlockPtr.setLastOp_spec,
+    Sim.OperationPtr.setNextOp_spec, Sim.OperationPtr.setPrevOp_spec,
+    Sim.OperationPtr.setParent_spec,
+    OpResultPtr.get!_BlockPtr_setFirstOp, OpResultPtr.get!_BlockPtr_setLastOp,
+    OpResultPtr.get!_OperationPtr_setNextOp, OpResultPtr.get!_OperationPtr_setPrevOp,
+    OpResultPtr.get!_OperationPtr_setParent]
+
+@[simp]
+theorem BlockArgumentPtr.get!_detachOp
+    (ctx : Sim.IRContext OpInfo) (op : Sim.OperationPtr)
+    (hctx : ctx.spec.FieldsInBounds) (hIn : op.InBounds ctx)
+    (hasParent : (op.getParent ctx hIn).toOption.isSome)
+    (argument : Veir.BlockArgumentPtr) :
+    argument.get! (Rewriter.detachOp ctx op hctx hIn hasParent).spec =
+      argument.get! ctx.spec := by
+  simp only [Rewriter.detachOp_def, Rewriter.detachOpSim,
+    Rewriter.unsetParentAndNeighbors_def, Rewriter.unsetParentAndNeighborsSim]
+  split <;> split
+  all_goals simp only [Sim.BlockPtr.setFirstOp_spec, Sim.BlockPtr.setLastOp_spec,
+    Sim.OperationPtr.setNextOp_spec, Sim.OperationPtr.setPrevOp_spec,
+    Sim.OperationPtr.setParent_spec,
+    BlockArgumentPtr.get!_BlockPtr_setFirstOp, BlockArgumentPtr.get!_BlockPtr_setLastOp,
+    BlockArgumentPtr.get!_OperationPtr_setNextOp,
+    BlockArgumentPtr.get!_OperationPtr_setPrevOp,
+    BlockArgumentPtr.get!_OperationPtr_setParent]
+
+@[simp]
+theorem RegionPtr.get!_detachOp
+    (ctx : Sim.IRContext OpInfo) (op : Sim.OperationPtr)
+    (hctx : ctx.spec.FieldsInBounds) (hIn : op.InBounds ctx)
+    (hasParent : (op.getParent ctx hIn).toOption.isSome)
+    (region : Veir.RegionPtr) :
+    region.get! (Rewriter.detachOp ctx op hctx hIn hasParent).spec =
+      region.get! ctx.spec := by
+  simp only [Rewriter.detachOp_def, Rewriter.detachOpSim,
+    Rewriter.unsetParentAndNeighbors_def, Rewriter.unsetParentAndNeighborsSim]
+  split <;> split
+  all_goals simp only [Sim.BlockPtr.setFirstOp_spec, Sim.BlockPtr.setLastOp_spec,
+    Sim.OperationPtr.setNextOp_spec, Sim.OperationPtr.setPrevOp_spec,
+    Sim.OperationPtr.setParent_spec,
+    RegionPtr.get!_BlockPtr_setFirstOp, RegionPtr.get!_BlockPtr_setLastOp,
+    RegionPtr.get!_OperationPtr_setNextOp, RegionPtr.get!_OperationPtr_setPrevOp,
+    RegionPtr.get!_OperationPtr_setParent]
+
+@[simp]
+theorem ValuePtr.getFirstUse!_detachOp
+    (ctx : Sim.IRContext OpInfo) (op : Sim.OperationPtr)
+    (hctx : ctx.spec.FieldsInBounds) (hIn : op.InBounds ctx)
+    (hasParent : (op.getParent ctx hIn).toOption.isSome)
+    (value : Veir.ValuePtr) :
+    value.getFirstUse! (Rewriter.detachOp ctx op hctx hIn hasParent).spec =
+      value.getFirstUse! ctx.spec := by
+  simp only [Rewriter.detachOp_def, Rewriter.detachOpSim,
+    Rewriter.unsetParentAndNeighbors_def, Rewriter.unsetParentAndNeighborsSim]
+  split <;> split
+  all_goals simp only [Sim.BlockPtr.setFirstOp_spec, Sim.BlockPtr.setLastOp_spec,
+    Sim.OperationPtr.setNextOp_spec, Sim.OperationPtr.setPrevOp_spec,
+    Sim.OperationPtr.setParent_spec,
+    ValuePtr.getFirstUse!_BlockPtr_setFirstOp, ValuePtr.getFirstUse!_BlockPtr_setLastOp,
+    ValuePtr.getFirstUse!_OperationPtr_setNextOp,
+    ValuePtr.getFirstUse!_OperationPtr_setPrevOp,
+    ValuePtr.getFirstUse!_OperationPtr_setParent]
+
+@[simp, grind =]
+theorem OperationPtr.getNumResults!_detachOp
+    (ctx : Sim.IRContext OpInfo) (op : Sim.OperationPtr)
+    (hctx : ctx.spec.FieldsInBounds) (hIn : op.InBounds ctx)
+    (hasParent : (op.getParent ctx hIn).toOption.isSome)
+    (operation : Veir.OperationPtr) :
+    operation.getNumResults! (Rewriter.detachOp ctx op hctx hIn hasParent).spec =
+      operation.getNumResults! ctx.spec := by
+  simp only [Rewriter.detachOp_def, Rewriter.detachOpSim,
+    Rewriter.unsetParentAndNeighbors_def, Rewriter.unsetParentAndNeighborsSim]
+  split <;> split
+  all_goals simp only [Sim.BlockPtr.setFirstOp_spec, Sim.BlockPtr.setLastOp_spec,
+    Sim.OperationPtr.setNextOp_spec, Sim.OperationPtr.setPrevOp_spec,
+    Sim.OperationPtr.setParent_spec]
+  all_goals grind
+
+@[simp, grind =]
+theorem OperationPtr.getNumRegions!_detachOp
+    (ctx : Sim.IRContext OpInfo) (op : Sim.OperationPtr)
+    (hctx : ctx.spec.FieldsInBounds) (hIn : op.InBounds ctx)
+    (hasParent : (op.getParent ctx hIn).toOption.isSome)
+    (operation : Veir.OperationPtr) :
+    operation.getNumRegions! (Rewriter.detachOp ctx op hctx hIn hasParent).spec =
+      operation.getNumRegions! ctx.spec := by
+  simp only [Rewriter.detachOp_def, Rewriter.detachOpSim,
+    Rewriter.unsetParentAndNeighbors_def, Rewriter.unsetParentAndNeighborsSim]
+  split <;> split
+  all_goals simp only [Sim.BlockPtr.setFirstOp_spec, Sim.BlockPtr.setLastOp_spec,
+    Sim.OperationPtr.setNextOp_spec, Sim.OperationPtr.setPrevOp_spec,
+    Sim.OperationPtr.setParent_spec]
+  all_goals grind
+
+@[simp, grind =]
+theorem OperationPtr.getRegion!_detachOp
+    (ctx : Sim.IRContext OpInfo) (op : Sim.OperationPtr)
+    (hctx : ctx.spec.FieldsInBounds) (hIn : op.InBounds ctx)
+    (hasParent : (op.getParent ctx hIn).toOption.isSome)
+    (operation : Veir.OperationPtr) (i : Nat) :
+    operation.getRegion! (Rewriter.detachOp ctx op hctx hIn hasParent).spec i =
+      operation.getRegion! ctx.spec i := by
+  simp only [Rewriter.detachOp_def, Rewriter.detachOpSim,
+    Rewriter.unsetParentAndNeighbors_def, Rewriter.unsetParentAndNeighborsSim]
+  split <;> split
+  all_goals simp only [Sim.BlockPtr.setFirstOp_spec, Sim.BlockPtr.setLastOp_spec,
+    Sim.OperationPtr.setNextOp_spec, Sim.OperationPtr.setPrevOp_spec,
+    Sim.OperationPtr.setParent_spec]
+  all_goals grind
+
+@[simp, grind =]
+theorem OperationPtr.capResults!_detachOp
+    (ctx : Sim.IRContext OpInfo) (op : Sim.OperationPtr)
+    (hctx : ctx.spec.FieldsInBounds) (hIn : op.InBounds ctx)
+    (hasParent : (op.getParent ctx hIn).toOption.isSome)
+    (operation : Veir.OperationPtr) :
+    (operation.get! (Rewriter.detachOp ctx op hctx hIn hasParent).spec).capResults =
+      (operation.get! ctx.spec).capResults := by
+  simp only [Rewriter.detachOp_def, Rewriter.detachOpSim,
+    Rewriter.unsetParentAndNeighbors_def, Rewriter.unsetParentAndNeighborsSim]
+  split <;> split
+  all_goals simp only [Sim.BlockPtr.setFirstOp_spec, Sim.BlockPtr.setLastOp_spec,
+    Sim.OperationPtr.setNextOp_spec, Sim.OperationPtr.setPrevOp_spec,
+    Sim.OperationPtr.setParent_spec]
+  all_goals grind
+
+@[simp, grind =]
+theorem OperationPtr.capRegions!_detachOp
+    (ctx : Sim.IRContext OpInfo) (op : Sim.OperationPtr)
+    (hctx : ctx.spec.FieldsInBounds) (hIn : op.InBounds ctx)
+    (hasParent : (op.getParent ctx hIn).toOption.isSome)
+    (operation : Veir.OperationPtr) :
+    (operation.get! (Rewriter.detachOp ctx op hctx hIn hasParent).spec).capRegions =
+      (operation.get! ctx.spec).capRegions := by
+  simp only [Rewriter.detachOp_def, Rewriter.detachOpSim,
+    Rewriter.unsetParentAndNeighbors_def, Rewriter.unsetParentAndNeighborsSim]
+  split <;> split
+  all_goals simp only [Sim.BlockPtr.setFirstOp_spec, Sim.BlockPtr.setLastOp_spec,
+    Sim.OperationPtr.setNextOp_spec, Sim.OperationPtr.setPrevOp_spec,
+    Sim.OperationPtr.setParent_spec]
+  all_goals grind
+
+@[simp, grind =]
+theorem BlockPtr.getNumArguments!_detachOp
+    (ctx : Sim.IRContext OpInfo) (op : Sim.OperationPtr)
+    (hctx : ctx.spec.FieldsInBounds) (hIn : op.InBounds ctx)
+    (hasParent : (op.getParent ctx hIn).toOption.isSome)
+    (block : Veir.BlockPtr) :
+    block.getNumArguments! (Rewriter.detachOp ctx op hctx hIn hasParent).spec =
+      block.getNumArguments! ctx.spec := by
+  simp only [Rewriter.detachOp_def, Rewriter.detachOpSim,
+    Rewriter.unsetParentAndNeighbors_def, Rewriter.unsetParentAndNeighborsSim]
+  split <;> split
+  all_goals simp only [Sim.BlockPtr.setFirstOp_spec, Sim.BlockPtr.setLastOp_spec,
+    Sim.OperationPtr.setNextOp_spec, Sim.OperationPtr.setPrevOp_spec,
+    Sim.OperationPtr.setParent_spec]
+  all_goals grind
+
+@[simp, grind =]
+theorem BlockPtr.capArguments!_detachOp
+    (ctx : Sim.IRContext OpInfo) (op : Sim.OperationPtr)
+    (hctx : ctx.spec.FieldsInBounds) (hIn : op.InBounds ctx)
+    (hasParent : (op.getParent ctx hIn).toOption.isSome)
+    (block : Veir.BlockPtr) :
+    (block.get! (Rewriter.detachOp ctx op hctx hIn hasParent).spec).capArguments =
+      (block.get! ctx.spec).capArguments := by
+  simp only [Rewriter.detachOp_def, Rewriter.detachOpSim,
+    Rewriter.unsetParentAndNeighbors_def, Rewriter.unsetParentAndNeighborsSim]
+  split <;> split
+  all_goals simp only [Sim.BlockPtr.setFirstOp_spec, Sim.BlockPtr.setLastOp_spec,
+    Sim.OperationPtr.setNextOp_spec, Sim.OperationPtr.setPrevOp_spec,
+    Sim.OperationPtr.setParent_spec]
+  all_goals grind
+
+@[simp]
+theorem BlockPtr.prev!_detachOp
+    (ctx : Sim.IRContext OpInfo) (op : Sim.OperationPtr)
+    (hctx : ctx.spec.FieldsInBounds) (hIn : op.InBounds ctx)
+    (hasParent : (op.getParent ctx hIn).toOption.isSome)
+    (block : Veir.BlockPtr) :
+    (block.get! (Rewriter.detachOp ctx op hctx hIn hasParent).spec).prev =
+      (block.get! ctx.spec).prev := by
+  simp only [Rewriter.detachOp_def, Rewriter.detachOpSim,
+    Rewriter.unsetParentAndNeighbors_def, Rewriter.unsetParentAndNeighborsSim]
+  split <;> split
+  all_goals simp only [Sim.BlockPtr.setFirstOp_spec, Sim.BlockPtr.setLastOp_spec,
+    Sim.OperationPtr.setNextOp_spec, Sim.OperationPtr.setPrevOp_spec,
+    Sim.OperationPtr.setParent_spec,
+    BlockPtr.prev!_BlockPtr_setFirstOp, BlockPtr.prev!_BlockPtr_setLastOp,
+    BlockPtr.get!_OperationPtr_setNextOp, BlockPtr.get!_OperationPtr_setPrevOp,
+    BlockPtr.get!_OperationPtr_setParent]
+
+@[simp]
+theorem BlockPtr.next!_detachOp
+    (ctx : Sim.IRContext OpInfo) (op : Sim.OperationPtr)
+    (hctx : ctx.spec.FieldsInBounds) (hIn : op.InBounds ctx)
+    (hasParent : (op.getParent ctx hIn).toOption.isSome)
+    (block : Veir.BlockPtr) :
+    (block.get! (Rewriter.detachOp ctx op hctx hIn hasParent).spec).next =
+      (block.get! ctx.spec).next := by
+  simp only [Rewriter.detachOp_def, Rewriter.detachOpSim,
+    Rewriter.unsetParentAndNeighbors_def, Rewriter.unsetParentAndNeighborsSim]
+  split <;> split
+  all_goals simp only [Sim.BlockPtr.setFirstOp_spec, Sim.BlockPtr.setLastOp_spec,
+    Sim.OperationPtr.setNextOp_spec, Sim.OperationPtr.setPrevOp_spec,
+    Sim.OperationPtr.setParent_spec,
+    BlockPtr.next!_BlockPtr_setFirstOp, BlockPtr.next!_BlockPtr_setLastOp,
+    BlockPtr.get!_OperationPtr_setNextOp, BlockPtr.get!_OperationPtr_setPrevOp,
+    BlockPtr.get!_OperationPtr_setParent]
+
+@[simp]
+theorem BlockPtr.parent!_detachOp
+    (ctx : Sim.IRContext OpInfo) (op : Sim.OperationPtr)
+    (hctx : ctx.spec.FieldsInBounds) (hIn : op.InBounds ctx)
+    (hasParent : (op.getParent ctx hIn).toOption.isSome)
+    (block : Veir.BlockPtr) :
+    (block.get! (Rewriter.detachOp ctx op hctx hIn hasParent).spec).parent =
+      (block.get! ctx.spec).parent := by
+  simp only [Rewriter.detachOp_def, Rewriter.detachOpSim,
+    Rewriter.unsetParentAndNeighbors_def, Rewriter.unsetParentAndNeighborsSim]
+  split <;> split
+  all_goals simp only [Sim.BlockPtr.setFirstOp_spec, Sim.BlockPtr.setLastOp_spec,
+    Sim.OperationPtr.setNextOp_spec, Sim.OperationPtr.setPrevOp_spec,
+    Sim.OperationPtr.setParent_spec,
+    BlockPtr.parent!_BlockPtr_setFirstOp, BlockPtr.parent!_BlockPtr_setLastOp,
+    BlockPtr.get!_OperationPtr_setNextOp, BlockPtr.get!_OperationPtr_setPrevOp,
+    BlockPtr.get!_OperationPtr_setParent]
+
+attribute [grind =] BlockPtr.firstUse!_detachOp BlockPtr.firstOp!_detachOp
+  BlockPtr.lastOp!_detachOp BlockPtr.prev!_detachOp BlockPtr.next!_detachOp
+  BlockPtr.parent!_detachOp OperationPtr.prev!_detachOp OperationPtr.next!_detachOp
+  OperationPtr.parent!_detachOp OpOperandPtr.get!_detachOp BlockOperandPtr.get!_detachOp
+  OpResultPtr.get!_detachOp BlockArgumentPtr.get!_detachOp RegionPtr.get!_detachOp
+  ValuePtr.getFirstUse!_detachOp
+
+theorem BlockPtr.opChain_detachOp_other
+    (ctx : Sim.IRContext OpInfo) (op : Sim.OperationPtr)
+    (hctx : ctx.spec.FieldsInBounds) (hIn : op.InBounds ctx)
+    (hasParent : (op.getParent ctx hIn).toOption.isSome)
+    (hWf : BlockPtr.OpChain block ctx.spec array)
+    (hWf' : BlockPtr.OpChain block' ctx.spec array')
+    (hParent : (op.spec.get! ctx.spec).parent = some block')
+    (hNe : block ≠ block') :
+    BlockPtr.OpChain block (Rewriter.detachOp ctx op hctx hIn hasParent).spec array := by
+  apply BlockPtr.OpChain_unchanged (ctx := ctx.spec) hWf <;>
+    grind [BlockPtr.OpChain]
+
+theorem BlockPtr.OpChain.prev_ne_self
+    (ctx : IRContext OpInfo) (block : BlockPtr) (array : Array OperationPtr)
+    (missingOps : Std.ExtHashSet OperationPtr) (op : OperationPtr)
+    (hWf : block.OpChain ctx array missingOps)
+    (hop : op.InBounds ctx)
+    (hmissing : op ∉ missingOps)
+    (hparent : (op.get! ctx).parent = some block) :
+    (op.get! ctx).prev ≠ some op := by
+  have opMem : op ∈ array := (hWf.allOpsInChain op hop hparent).mpr hmissing
+  intro heq
+  have ⟨i, hi⟩ := Array.getElem_of_mem opMem
+  have hopEq : array[i]'(by grind) = op := by grind
+  have hiPos : i > 0 := by grind [BlockPtr.OpChain]
+  have hprev := hWf.prev i hiPos (by grind)
+  have : op = array[i - 1]'(by grind) := by grind
+  grind [BlockPtr.OpChain_array_injective]
+
+theorem BlockPtr.OpChain.next_ne_self
+    (ctx : IRContext OpInfo) (block : BlockPtr) (array : Array OperationPtr)
+    (missingOps : Std.ExtHashSet OperationPtr) (op : OperationPtr)
+    (hWf : block.OpChain ctx array missingOps)
+    (hop : op.InBounds ctx)
+    (hmissing : op ∉ missingOps)
+    (hparent : (op.get! ctx).parent = some block) :
+    (op.get! ctx).next ≠ some op := by
+  have opMem : op ∈ array := (hWf.allOpsInChain op hop hparent).mpr hmissing
+  intro heq
+  have ⟨i, hi⟩ := Array.getElem?_of_mem opMem
+  have hnext : array[i + 1]? = some op := by grind [BlockPtr.OpChain]
+  grind [BlockPtr.OpChain_array_injective]
+
+set_option maxHeartbeats 800000 in
+theorem BlockPtr.opChain_detachOp_self
+    (ctx : Sim.IRContext OpInfo) (op : Sim.OperationPtr)
+    (hctx : ctx.spec.FieldsInBounds) (hIn : op.InBounds ctx)
+    (hasParent : (op.getParent ctx hIn).toOption.isSome)
+    (hWf : BlockPtr.OpChain block ctx.spec array)
+    (hParent : (op.spec.get! ctx.spec).parent = some block) :
+    BlockPtr.OpChain block (Rewriter.detachOp ctx op hctx hIn hasParent).spec
+      (array.erase op.spec) := by
+  have opInArray : op.spec ∈ array := by grind [BlockPtr.OpChain]
+  have ⟨i, iInBounds, hi⟩ := Array.getElem_of_mem opInArray
+  constructor
+  case prev =>
+    rw [← hi]
+    intros i' hi₁' hi₂'
+    simp only [BlockPtr.OpChain.erase_getElem_array_eq_eraseIdx hWf]
+    by_cases i' < i
+    · simp (disch := grind) only [Array.getElem_eraseIdx_of_lt]
+      simp only [OperationPtr.prev!_detachOp]
+      grind (instances := 2000) [BlockPtr.OpChain, BlockPtr.OpChain_array_injective]
+    · by_cases i' = i
+      · grind [BlockPtr.OpChain, BlockPtr.OpChain_array_injective]
+      · grind [BlockPtr.OpChain, BlockPtr.OpChain_array_injective]
+  case next =>
+    rw [← hi]
+    intros i' hi'
+    simp only [BlockPtr.OpChain.erase_getElem_array_eq_eraseIdx hWf]
+    by_cases i' > i
+    · simp (disch := grind) only [Array.getElem_eraseIdx_of_ge,
+        Array.getElem?_eraseIdx_of_ge]
+      simp only [OperationPtr.next!_detachOp]
+      grind [BlockPtr.OpChain, BlockPtr.OpChain_array_injective]
+    · by_cases i' = i
+      · grind [BlockPtr.OpChain, BlockPtr.OpChain_array_injective]
+      · grind [BlockPtr.OpChain, BlockPtr.OpChain_array_injective]
+  all_goals grind [BlockPtr.OpChain]
+
+theorem ValuePtr.defUse_detachOp
+    (ctx : Sim.IRContext OpInfo) (op : Sim.OperationPtr)
+    (hctx : ctx.spec.FieldsInBounds) (hIn : op.InBounds ctx)
+    (hasParent : (op.getParent ctx hIn).toOption.isSome)
+    (hWf : ValuePtr.DefUse value ctx.spec array missingUses) :
+    ValuePtr.DefUse value (Rewriter.detachOp ctx op hctx hIn hasParent).spec
+      array missingUses := by
+  apply ValuePtr.DefUse.unchanged (ctx := ctx.spec) <;> grind
+
+theorem BlockPtr.defUse_detachOp
+    (ctx : Sim.IRContext OpInfo) (op : Sim.OperationPtr)
+    (hctx : ctx.spec.FieldsInBounds) (hIn : op.InBounds ctx)
+    (hasParent : (op.getParent ctx hIn).toOption.isSome)
+    (hWf : BlockPtr.DefUse block ctx.spec array missingUses) :
+    BlockPtr.DefUse block (Rewriter.detachOp ctx op hctx hIn hasParent).spec
+      array missingUses := by
+  apply BlockPtr.DefUse.unchanged (ctx := ctx.spec) <;> grind
+
+theorem RegionPtr.blockChain_detachOp
+    (ctx : Sim.IRContext OpInfo) (op : Sim.OperationPtr)
+    (hctx : ctx.spec.FieldsInBounds) (hIn : op.InBounds ctx)
+    (hasParent : (op.getParent ctx hIn).toOption.isSome)
+    (hWf : RegionPtr.BlockChain region ctx.spec array) :
+    RegionPtr.BlockChain region (Rewriter.detachOp ctx op hctx hIn hasParent).spec array := by
+  apply RegionPtr.blockChain_unchanged (ctx := ctx.spec) hWf <;> grind
+
+theorem Rewriter.detachOp_WellFormed
+    (ctx : Sim.IRContext OpInfo)
+    (wf : ctx.spec.WellFormed missingOperands missingSuccessors)
+    (hctx : ctx.spec.FieldsInBounds) (op : Sim.OperationPtr)
+    (hIn : op.InBounds ctx)
+    (hasParent : (op.getParent ctx hIn).toOption.isSome) :
+    (Rewriter.detachOp ctx op hctx hIn hasParent).spec.WellFormed
+      missingOperands missingSuccessors := by
+  have hParentIB : (op.getParent ctx hIn).InBounds ctx := by grind
+  have hParentSome : (op.getParent ctx hIn).spec =
+      some ((op.getParent ctx hIn).toOption.get hasParent).spec := by
+    apply Sim.OptionBlockPtr.toOption_some hParentIB
+    exact (Option.some_get hasParent).symm
+  rw [Sim.OperationPtr.getParent_spec ctx op hIn] at hParentSome
+  have hParent : (op.spec.get! ctx.spec).parent =
+      some ((op.getParent ctx hIn).toOption.get hasParent).spec := by
+    rw [OperationPtr.get!_eq_get]
+    exact hParentSome
+  constructor
+  case inBounds => exact Rewriter.detachOp_fieldsInBounds hctx
+  case valueDefUseChains =>
+    intro value hvalue
+    have ⟨array, harray⟩ := wf.valueDefUseChains value (by grind)
+    refine ⟨array, ?_⟩
+    apply ValuePtr.defUse_detachOp ctx op hctx hIn hasParent
+    apply cast (a := harray)
+    congr
+    ext use
+    rw [OpOperandPtr.get!_detachOp]
+  case blockDefUseChains =>
+    intro block hblock
+    have ⟨array, harray⟩ := wf.blockDefUseChains block (by grind)
+    refine ⟨array, ?_⟩
+    apply BlockPtr.defUse_detachOp ctx op hctx hIn hasParent
+    apply cast (a := harray)
+    congr
+    ext use
+    rw [BlockOperandPtr.get!_detachOp]
+  case opChain =>
+    intro block' hBlock'
+    have ⟨array', harray'⟩ := wf.opChain block' (by grind)
+    let block := ((op.getParent ctx hIn).toOption.get hasParent).spec
+    by_cases hEq : block = block'
+    · subst block'
+      exact ⟨array'.erase op.spec,
+        BlockPtr.opChain_detachOp_self ctx op hctx hIn hasParent harray' hParent⟩
+    · have ⟨array, harray⟩ := wf.opChain block (by grind)
+      exact ⟨array', BlockPtr.opChain_detachOp_other ctx op hctx hIn hasParent
+        harray' harray hParent (Ne.symm hEq)⟩
+  case blockChain =>
+    intro region hregion
+    have ⟨array, harray⟩ := wf.blockChain region (by grind)
+    exact ⟨array, RegionPtr.blockChain_detachOp ctx op hctx hIn hasParent harray⟩
+  case operations =>
+    intro op' hop'
+    have hopOld : op'.InBounds ctx.spec := by grind
+    have hWf := wf.operations op' hopOld
+    constructor
+    case inBounds => grind
+    case result_index =>
+      intro i hi
+      have hi' : i < op'.getNumResults! ctx.spec := by simpa using hi
+      simpa using hWf.result_index i hi'
+    case result_owner =>
+      intro i hi
+      have hi' : i < op'.getNumResults! ctx.spec := by simpa using hi
+      simpa using hWf.result_owner i hi'
+    case operand_owner =>
+      intro i hi
+      rw [Rewriter.detachOp_preserves_numOperands hctx] at hi
+      simpa using hWf.operand_owner i hi
+    case blockOperand_owner =>
+      intro i hi
+      rw [Rewriter.detachOp_preserves_numSuccessors hctx] at hi
+      simpa using hWf.blockOperand_owner i hi
+    case regions_unique =>
+      intro i hi j hj hne
+      have hi' : i < op'.getNumRegions! ctx.spec := by simpa using hi
+      have hj' : j < op'.getNumRegions! ctx.spec := by simpa using hj
+      intro heq
+      have heqBang : op'.getRegion!
+          (Rewriter.detachOp ctx op hctx hIn hasParent).spec i =
+          op'.getRegion! (Rewriter.detachOp ctx op hctx hIn hasParent).spec j := by
+        rw [OperationPtr.getRegion!_eq_getRegion
+          (ctx := (Rewriter.detachOp ctx op hctx hIn hasParent).spec)
+          (op := op') (index := i) (hin := hop') (iInBounds := by grind),
+          OperationPtr.getRegion!_eq_getRegion
+          (ctx := (Rewriter.detachOp ctx op hctx hIn hasParent).spec)
+          (op := op') (index := j) (hin := hop') (iInBounds := by grind)]
+        exact heq
+      rw [OperationPtr.getRegion!_detachOp, OperationPtr.getRegion!_detachOp] at heqBang
+      apply hWf.regions_unique i hi' j hj' hne
+      rw [← OperationPtr.getRegion!_eq_getRegion
+          (ctx := ctx.spec) (op := op') (index := i) (hin := hopOld)
+          (iInBounds := by grind),
+        ← OperationPtr.getRegion!_eq_getRegion
+          (ctx := ctx.spec) (op := op') (index := j) (hin := hopOld)
+          (iInBounds := by grind)]
+      exact heqBang
+    case region_parent =>
+      intro region regionInBounds
+      have regionOld : region.InBounds ctx.spec := by grind
+      simpa using hWf.region_parent region regionOld
+    case opChain_of_parent_none =>
+      have ⟨chain, hchain⟩ := wf.opChain
+        ((op.getParent ctx hIn).toOption.get hasParent).spec (by grind)
+      intro hnone
+      rw [OperationPtr.prev!_detachOp, OperationPtr.next!_detachOp]
+      by_cases heq : op' = op.spec
+      · subst op'
+        have hPrevNe := BlockPtr.OpChain.prev_ne_self _ _ _ _ _ hchain hIn.ib
+          (by simp) hParent
+        have hNextNe := BlockPtr.OpChain.next_ne_self _ _ _ _ _ hchain hIn.ib
+          (by simp) hParent
+        simp [Ne.symm hNextNe, Ne.symm hPrevNe]
+      · have hOldParent : (op'.get! ctx.spec).parent = none := by
+          rw [OperationPtr.parent!_detachOp] at hnone
+          simpa [heq] using hnone
+        have hold := hWf.opChain_of_parent_none hOldParent
+        grind [BlockPtr.OpChain_next_ne, BlockPtr.OpChain_prev_ne]
+    case capResults_eq_numResults => simpa using hWf.capResults_eq_numResults
+    case capRegions_eq_numRegions => simpa using hWf.capRegions_eq_numRegions
+    case capOperands_eq_numOperands =>
+      simpa only [Rewriter.detachOp_preserves_capOperands hctx,
+        Rewriter.detachOp_preserves_numOperands hctx] using hWf.capOperands_eq_numOperands
+    case capBlockOperands_eq_numSuccessors =>
+      simpa only [Rewriter.detachOp_preserves_capBlockOperands hctx,
+        Rewriter.detachOp_preserves_numSuccessors hctx] using
+          hWf.capBlockOperands_eq_numSuccessors
+  case blocks =>
+    intro block hblock
+    have hWf := wf.blocks block (by grind)
+    apply BlockPtr.WellFormed_unchanged (ctx := ctx.spec) <;> grind
+  case regions =>
+    intro region hregion
+    have hWf := wf.regions region (by grind)
+    apply RegionPtr.WellFormed_unchanged (ctx := ctx.spec) <;> grind
+
+theorem Rewriter.detachOpIfAttached_WellFormed
+    (ctx : Sim.IRContext OpInfo)
+    (wf : ctx.spec.WellFormed missingOperands missingSuccessors)
+    (hctx : ctx.spec.FieldsInBounds) (op : Sim.OperationPtr)
+    (hIn : op.InBounds ctx) :
+    (Rewriter.detachOpIfAttached ctx op hctx hIn).spec.WellFormed
+      missingOperands missingSuccessors := by
+  simp only [Rewriter.detachOpIfAttached_def, Rewriter.detachOpIfAttachedSim]
+  split
+  · apply Rewriter.detachOp_WellFormed <;> assumption
+  · exact wf
+
+theorem Rewriter.detachOperands_wellFormed
+    (ctx : Sim.IRContext OpInfo) (op : Sim.OperationPtr)
+    (hCtx : ctx.spec.FieldsInBounds) (hOp : op.InBounds ctx)
+    (hCap : (op.spec.get! ctx.spec).capOperands =
+      op.spec.getNumOperands! ctx.spec)
+    (wf : ctx.spec.WellFormed missingOperands missingSuccessors)
+    (hMissing : ∀ i, OpOperandPtr.mk op.spec i ∉ missingOperands) :
+    (Rewriter.detachOperands ctx op hCtx hOp hCap).spec.WellFormed
+      (missingOperands.insertMany
+        ((0...op.spec.getNumOperands! ctx.spec).toList.map
+          (fun i => OpOperandPtr.mk op.spec i)))
+      missingSuccessors := by
+  let numOperands := op.getNumOperands ctx hOp
+  have hNumLt : op.spec.getNumOperands! ctx.spec < UInt64.size := by
+    have henc := ctx.sim.encoding_op op.spec hOp.ib
+    rw [← hCap, henc.numOperands]
+    exact UInt64.toNat_lt _
+  have hNum : numOperands.toNat = op.spec.getNumOperands! ctx.spec := by
+    dsimp [numOperands]
+    rw [Sim.OperationPtr.getNumOperands_eq_getNumOperands! ctx op hOp,
+      Sim.OperationPtr.getNumOperands!_spec (ctx := ctx) op (ib := hOp), hCap]
+    exact UInt64.toNat_ofNat_of_lt hNumLt
+  simp only [Rewriter.detachOperands_def, Rewriter.detachOperandsSim]
+  split
+  next hz =>
+    have hZero : op.spec.getNumOperands! ctx.spec = 0 := by
+      rw [← hNum]
+      exact congrArg UInt64.toNat hz
+    simpa [hZero] using wf
+  next hz =>
+    have hPos : 0 < numOperands.toNat := by
+      have hneNat : numOperands.toNat ≠ 0 := by
+        intro hzero
+        apply hz
+        apply UInt64.toNat_inj.mp
+        simpa using hzero
+      omega
+    have hNumBound := UInt64.toNat_lt numOperands
+    have hPred : (numOperands - 1).toNat = numOperands.toNat - 1 := by
+      rw [UInt64.toNat_sub]
+      change (2 ^ 64 - 1 + numOperands.toNat) % 2 ^ 64 = numOperands.toNat - 1
+      have heq : 2 ^ 64 - 1 + numOperands.toNat =
+          2 ^ 64 + (numOperands.toNat - 1) := by omega
+      rw [heq, Nat.add_mod]
+      simp only [Nat.mod_self, Nat.zero_add]
+      rw [Nat.mod_eq_of_lt (by omega), Nat.mod_eq_of_lt (by omega)]
+    have hwfLoop := Rewriter.detachOperands.loop_wellFormed
+      (ctx := ctx) (op := op) (off := op.getOperandsOffset ctx (by grind))
+      (index := numOperands - 1) (hCtx := hCtx) (hOp := hOp)
+      (hIndex := by rw [hPred, hNum]; omega) (hoff := by grind) (wf := wf)
+      (hMissing := by
+        intro i hi
+        exact hMissing i)
+    have hRange :
+        ((0...=(numOperands - 1).toNat).toList.map
+          (fun i => OpOperandPtr.mk op.spec i)) =
+        ((0...op.spec.getNumOperands! ctx.spec).toList.map
+          (fun i => OpOperandPtr.mk op.spec i)) := by
+      rw [Nat.toList_rcc_eq_toList_rco, hPred, hNum]
+      have hSucc : op.spec.getNumOperands! ctx.spec - 1 + 1 =
+          op.spec.getNumOperands! ctx.spec := by omega
+      rw [hSucc]
+    rw [hRange] at hwfLoop
+    exact hwfLoop
+
+theorem Rewriter.detachBlockOperands.loop_wellFormed
+    (ctx : Sim.IRContext OpInfo) (op : Sim.OperationPtr) (index : UInt64)
+    (hCtx : ctx.spec.FieldsInBounds) (hOp : op.InBounds ctx)
+    (hIndex : index.toNat < op.spec.getNumSuccessors! ctx.spec)
+    (wf : ctx.spec.WellFormed missingOperands missingSuccessors)
+    (hMissing : ∀ i, i ≤ index.toNat →
+      BlockOperandPtr.mk op.spec i ∉ missingSuccessors) :
+    (Rewriter.detachBlockOperands.loop ctx op index hCtx hOp hIndex).spec.WellFormed
+      missingOperands
+      (missingSuccessors.insertMany
+        ((0...=index.toNat).toList.map (fun i => BlockOperandPtr.mk op.spec i))) := by
+  simp only [Rewriter.detachBlockOperands.loop_def]
+  fun_induction Rewriter.detachBlockOperands.loopSim generalizing missingOperands missingSuccessors
+  case case1 =>
+    let use := op.getBlockOperandPtr _ 0 (by assumption)
+    have hUseSpec : use.spec = BlockOperandPtr.mk op.spec 0 := rfl
+    have hwf := Sim.IRContext.wellFormed_BlockOperandPtr_removeFromCurrent
+      (use := use) (useInBounds := by
+        dsimp [use]
+        exact Sim.OperationPtr.getBlockOperand_inBounds op (by assumption) 0 (by assumption))
+      (ctxInBounds := wf.inBounds)
+      (useMissing := by simpa [hUseSpec] using hMissing 0 (by simp)) wf
+    simpa [use, hUseSpec, Nat.toList_rcc_eq_singleton,
+      Std.ExtHashSet.insertMany_list_singleton] using hwf
+  case case2 =>
+    rename_i _ _ _ currentCtx currentIndex hCtxCur hOpCur hIndexCur currentCtx' hne ih
+    have hCurrentPos : 0 < currentIndex.toNat := by
+      have hneNat : currentIndex.toNat ≠ 0 := by
+        intro hz
+        apply hne
+        apply UInt64.toNat_inj.mp
+        simpa using hz
+      omega
+    have hCurrentLt := UInt64.toNat_lt currentIndex
+    have hPred : (currentIndex - 1).toNat = currentIndex.toNat - 1 := by
+      rw [UInt64.toNat_sub]
+      change (2 ^ 64 - 1 + currentIndex.toNat) % 2 ^ 64 = currentIndex.toNat - 1
+      have heq : 2 ^ 64 - 1 + currentIndex.toNat =
+          2 ^ 64 + (currentIndex.toNat - 1) := by omega
+      rw [heq, Nat.add_mod]
+      simp only [Nat.mod_self, Nat.zero_add]
+      rw [Nat.mod_eq_of_lt (by omega), Nat.mod_eq_of_lt (by omega)]
+    let use := op.getBlockOperandPtr currentCtx currentIndex (by assumption)
+    have hUseSpec : use.spec = BlockOperandPtr.mk op.spec currentIndex.toNat := rfl
+    have hwfRemoved := Sim.IRContext.wellFormed_BlockOperandPtr_removeFromCurrent
+      (use := use) (useInBounds := by
+        dsimp [use]
+        exact Sim.OperationPtr.getBlockOperand_inBounds op (by assumption) currentIndex
+          (by assumption))
+      (ctxInBounds := wf.inBounds)
+      (useMissing := by
+        rw [hUseSpec]
+        exact hMissing currentIndex.toNat (Nat.le_refl _)) wf
+    have hwfRec := ih hwfRemoved (by
+      intro i hi
+      simp only [Std.ExtHashSet.mem_insert, hUseSpec, not_or]
+      constructor
+      · simp only [beq_iff_eq, BlockOperandPtr.mk.injEq, true_and]
+        rw [hPred] at hi
+        omega
+      · apply hMissing i
+        rw [hPred] at hi
+        omega)
+    have hSets :
+        (missingSuccessors.insert use.spec).insertMany
+            ((0...=(currentIndex - 1).toNat).toList.map
+              (fun i => BlockOperandPtr.mk op.spec i)) =
+          missingSuccessors.insertMany
+            ((0...=currentIndex.toNat).toList.map
+              (fun i => BlockOperandPtr.mk op.spec i)) := by
+      rw [hUseSpec, Nat.toList_rcc_eq_toList_rco, hPred]
+      have hSucc : currentIndex.toNat - 1 + 1 = currentIndex.toNat := by omega
+      rw [hSucc, Nat.toList_rcc_eq_append (Nat.zero_le _), List.map_append,
+        List.map_singleton, Std.ExtHashSet.insertMany_append,
+        Std.ExtHashSet.insertMany_list_singleton,
+        Std.ExtHashSet.insertMany_list_insert_comm]
+    rw [hSets] at hwfRec
+    exact hwfRec
+
+theorem Rewriter.detachBlockOperands_wellFormed
+    (ctx : Sim.IRContext OpInfo) (op : Sim.OperationPtr)
+    (hCtx : ctx.spec.FieldsInBounds) (hOp : op.InBounds ctx)
+    (hCap : (op.spec.get! ctx.spec).capBlockOperands =
+      op.spec.getNumSuccessors! ctx.spec)
+    (wf : ctx.spec.WellFormed missingOperands missingSuccessors)
+    (hMissing : ∀ i, BlockOperandPtr.mk op.spec i ∉ missingSuccessors) :
+    (Rewriter.detachBlockOperands ctx op hCtx hOp hCap).spec.WellFormed
+      missingOperands
+      (missingSuccessors.insertMany
+        ((0...op.spec.getNumSuccessors! ctx.spec).toList.map
+          (fun i => BlockOperandPtr.mk op.spec i))) := by
+  let numSuccessors := op.getNumSuccessors ctx hOp
+  have hNumLt : op.spec.getNumSuccessors! ctx.spec < UInt64.size := by
+    have henc := ctx.sim.encoding_op op.spec hOp.ib
+    rw [← hCap, henc.numBlockOperands]
+    exact UInt64.toNat_lt _
+  have hNum : numSuccessors.toNat = op.spec.getNumSuccessors! ctx.spec := by
+    dsimp [numSuccessors]
+    rw [Sim.OperationPtr.getNumSuccessors_eq_getNumSuccessors! ctx op hOp,
+      Sim.OperationPtr.getNumSuccessors!_spec (ctx := ctx) op (ib := hOp), hCap]
+    exact UInt64.toNat_ofNat_of_lt hNumLt
+  simp only [Rewriter.detachBlockOperands_def, Rewriter.detachBlockOperandsSim]
+  split
+  next hz =>
+    have hZero : op.spec.getNumSuccessors! ctx.spec = 0 := by
+      rw [← hNum]
+      exact congrArg UInt64.toNat hz
+    simpa [hZero] using wf
+  next hz =>
+    have hPos : 0 < numSuccessors.toNat := by
+      have hneNat : numSuccessors.toNat ≠ 0 := by
+        intro hzero
+        apply hz
+        apply UInt64.toNat_inj.mp
+        simpa using hzero
+      omega
+    have hNumBound := UInt64.toNat_lt numSuccessors
+    have hPred : (numSuccessors - 1).toNat = numSuccessors.toNat - 1 := by
+      rw [UInt64.toNat_sub]
+      change (2 ^ 64 - 1 + numSuccessors.toNat) % 2 ^ 64 = numSuccessors.toNat - 1
+      have heq : 2 ^ 64 - 1 + numSuccessors.toNat =
+          2 ^ 64 + (numSuccessors.toNat - 1) := by omega
+      rw [heq, Nat.add_mod]
+      simp only [Nat.mod_self, Nat.zero_add]
+      rw [Nat.mod_eq_of_lt (by omega), Nat.mod_eq_of_lt (by omega)]
+    have hwfLoop := Rewriter.detachBlockOperands.loop_wellFormed
+      (ctx := ctx) (op := op) (index := numSuccessors - 1)
+      (hCtx := hCtx) (hOp := hOp)
+      (hIndex := by rw [hPred, hNum]; omega) (wf := wf)
+      (hMissing := by
+        intro i hi
+        exact hMissing i)
+    have hRange :
+        ((0...=(numSuccessors - 1).toNat).toList.map
+          (fun i => BlockOperandPtr.mk op.spec i)) =
+        ((0...op.spec.getNumSuccessors! ctx.spec).toList.map
+          (fun i => BlockOperandPtr.mk op.spec i)) := by
+      rw [Nat.toList_rcc_eq_toList_rco, hPred, hNum]
+      have hSucc : op.spec.getNumSuccessors! ctx.spec - 1 + 1 =
+          op.spec.getNumSuccessors! ctx.spec := by omega
+      rw [hSucc]
+    rw [hRange] at hwfLoop
+    exact hwfLoop
+
+theorem OpResultPtr.firstUse!_OpOperandPtr_removeFromCurrent_eq_none_of_firstUse!_eq_none
+    (ctx : Sim.IRContext OpInfo) (operand : Sim.OpOperandPtr)
+    (operandIn : operand.InBounds ctx) (ctxIn : ctx.spec.FieldsInBounds)
+    (result : Veir.OpResultPtr)
+    (hctx : ctx.spec.WellFormed missingUses missingSuccessors)
+    (hmissing : operand.spec ∉ missingUses)
+    (resultIn : result.InBounds ctx.spec)
+    (h : (result.get! ctx.spec).firstUse = none) :
+    (result.get! (operand.removeFromCurrent ctx operandIn ctxIn).spec).firstUse = none := by
+  have ⟨useArray, hUseArray⟩ := hctx.valueDefUseChains (result : ValuePtr) (by grind)
+  have ⟨useArray', hUseArray'⟩ := hctx.valueDefUseChains
+    (operand.spec.get! ctx.spec).value (by grind)
+  have hne : (result : ValuePtr) ≠ (operand.spec.get! ctx.spec).value := by
+    grind [ValuePtr.DefUse]
+  have hEmpty : useArray = #[] := by
+    grind [ValuePtr.DefUse.getFirstUse!_none_iff hUseArray]
+  have operandInArray : operand.spec ∈ useArray' := by
+    grind [ValuePtr.DefUse]
+  have hPreserved := Sim.ValuePtr.defUse_removeFromCurrent_other hne
+    (useIb := operandIn) hUseArray hUseArray'
+    (hvalue := operandInArray) (ctxInBounds := hctx.inBounds)
+  grind [ValuePtr.DefUse.getFirstUse!_none_iff hPreserved]
+
+theorem OpResultPtr.firstUse!_detachOperands_loop_eq_none_of_firstUse!_eq_none
+    (ctx : Sim.IRContext OpInfo) (operation : Sim.OperationPtr)
+    (off : Int64) (index : UInt64) (result : Veir.OpResultPtr)
+    (hCtx : ctx.spec.FieldsInBounds) (hOp : operation.InBounds ctx)
+    (hIndex : index.toNat < operation.spec.getNumOperands! ctx.spec)
+    (hoff : off = Buffed.Operation.Offsets.operands operation.spec ctx.spec)
+    (hctx : ctx.spec.WellFormed missingUses missingSuccessors)
+    (hMissingUses : ∀ i, i ≤ index.toNat →
+      OpOperandPtr.mk operation.spec i ∉ missingUses)
+    (resIn : result.InBounds ctx.spec)
+    (h : (result.get! ctx.spec).firstUse = none) :
+    (result.get! (Rewriter.detachOperands.loop ctx operation off index
+      hCtx hOp hIndex hoff).spec).firstUse = none := by
+  simp only [Rewriter.detachOperands.loop_def]
+  fun_induction Rewriter.detachOperands.loopSim generalizing missingUses missingSuccessors
+  case case1 =>
+    let use := operation.getOperandPtrAt _ off 0 (by assumption) (by assumption)
+    have hUseSpec : use.spec = OpOperandPtr.mk operation.spec 0 := rfl
+    apply OpResultPtr.firstUse!_OpOperandPtr_removeFromCurrent_eq_none_of_firstUse!_eq_none
+      (ctx := _) (operand := use) (result := result)
+      (operandIn := by
+        dsimp [use]
+        rw [Sim.OperationPtr.getOperandPtrAt_eq_getOperandPtr]
+        exact Sim.OperationPtr.getOpOperand_inBounds operation (by assumption) 0
+          (by assumption))
+      (ctxIn := hctx.inBounds) hctx
+    · rw [hUseSpec]
+      exact hMissingUses 0 (by simp)
+    · exact resIn
+    · exact h
+  case case2 =>
+    rename_i _ _ _ currentCtx currentIndex hCtxCur hOpCur hIndexCur hoffCur currentCtx' hne ih
+    have hCurrentPos : 0 < currentIndex.toNat := by
+      have hneNat : currentIndex.toNat ≠ 0 := by
+        intro hz
+        apply hne
+        apply UInt64.toNat_inj.mp
+        simpa using hz
+      omega
+    have hCurrentLt := UInt64.toNat_lt currentIndex
+    have hPred : (currentIndex - 1).toNat = currentIndex.toNat - 1 := by
+      rw [UInt64.toNat_sub]
+      change (2 ^ 64 - 1 + currentIndex.toNat) % 2 ^ 64 = currentIndex.toNat - 1
+      have heq : 2 ^ 64 - 1 + currentIndex.toNat =
+          2 ^ 64 + (currentIndex.toNat - 1) := by omega
+      rw [heq, Nat.add_mod]
+      simp only [Nat.mod_self, Nat.zero_add]
+      rw [Nat.mod_eq_of_lt (by omega), Nat.mod_eq_of_lt (by omega)]
+    let use := operation.getOperandPtrAt currentCtx off currentIndex
+      (by assumption) (by assumption)
+    have hUseSpec : use.spec = OpOperandPtr.mk operation.spec currentIndex.toNat := rfl
+    have hUseIn : use.InBounds currentCtx := by
+      dsimp [use]
+      rw [Sim.OperationPtr.getOperandPtrAt_eq_getOperandPtr]
+      exact Sim.OperationPtr.getOpOperand_inBounds operation (by assumption) currentIndex
+        (by assumption)
+    have hwfRemoved := Sim.IRContext.wellFormed_OpOperandPtr_removeFromCurrent
+      (use := use) (useInBounds := hUseIn) (ctxInBounds := hctx.inBounds)
+      (useMissing := by
+        rw [hUseSpec]
+        exact hMissingUses currentIndex.toNat (Nat.le_refl _)) hctx
+    have hNoneRemoved :=
+      OpResultPtr.firstUse!_OpOperandPtr_removeFromCurrent_eq_none_of_firstUse!_eq_none
+        (ctx := currentCtx) (operand := use) (result := result)
+        (operandIn := hUseIn) (ctxIn := hctx.inBounds) hctx
+        (by rw [hUseSpec]; exact hMissingUses currentIndex.toNat (Nat.le_refl _))
+        resIn h
+    apply ih hwfRemoved
+    · intro i hi
+      simp only [Std.ExtHashSet.mem_insert, hUseSpec, not_or]
+      constructor
+      · simp only [beq_iff_eq, OpOperandPtr.mk.injEq, true_and]
+        rw [hPred] at hi
+        omega
+      · apply hMissingUses i
+        rw [hPred] at hi
+        omega
+    · grind
+    · exact hNoneRemoved
+
+theorem OpResultPtr.firstUse!_detachOperands_eq_none_of_firstUse!_eq_none
+    (ctx : Sim.IRContext OpInfo) (operation : Sim.OperationPtr)
+    (result : Veir.OpResultPtr)
+    (hCtx : ctx.spec.FieldsInBounds) (hOp : operation.InBounds ctx)
+    (hCap : (operation.spec.get! ctx.spec).capOperands =
+      operation.spec.getNumOperands! ctx.spec)
+    (hctx : ctx.spec.WellFormed missingUses missingSuccessors)
+    (hMissingUses : ∀ i, OpOperandPtr.mk operation.spec i ∉ missingUses)
+    (resIn : result.InBounds ctx.spec)
+    (h : (result.get! ctx.spec).firstUse = none) :
+    (result.get! (Rewriter.detachOperands ctx operation hCtx hOp hCap).spec).firstUse = none := by
+  let numOperands := operation.getNumOperands ctx hOp
+  have hNumLt : operation.spec.getNumOperands! ctx.spec < UInt64.size := by
+    have henc := ctx.sim.encoding_op operation.spec hOp.ib
+    rw [← hCap, henc.numOperands]
+    exact UInt64.toNat_lt _
+  have hNum : numOperands.toNat = operation.spec.getNumOperands! ctx.spec := by
+    dsimp [numOperands]
+    rw [Sim.OperationPtr.getNumOperands_eq_getNumOperands! ctx operation hOp,
+      Sim.OperationPtr.getNumOperands!_spec (ctx := ctx) operation (ib := hOp), hCap]
+    exact UInt64.toNat_ofNat_of_lt hNumLt
+  simp only [Rewriter.detachOperands_def, Rewriter.detachOperandsSim]
+  split
+  · exact h
+  · apply OpResultPtr.firstUse!_detachOperands_loop_eq_none_of_firstUse!_eq_none
+      (hctx := hctx) (hMissingUses := by intro i hi; exact hMissingUses i)
+      (resIn := resIn) (h := h)
+
+@[simp]
+theorem OpResultPtr.firstUse!_detachBlockOperands_loop
+    (ctx : Sim.IRContext OpInfo) (operation : Sim.OperationPtr)
+    (index : UInt64) (result : Veir.OpResultPtr)
+    (hCtx : ctx.spec.FieldsInBounds) (hOp : operation.InBounds ctx)
+    (hIndex : index.toNat < operation.spec.getNumSuccessors! ctx.spec) :
+    (result.get! (Rewriter.detachBlockOperands.loop ctx operation index
+      hCtx hOp hIndex).spec).firstUse = (result.get! ctx.spec).firstUse := by
+  simp only [Rewriter.detachBlockOperands.loop_def]
+  fun_induction Rewriter.detachBlockOperands.loopSim
+  case case1 =>
+    rename_i _ _ _ currentCtx hCtxCur hOpCur hIndexCur currentCtx'
+    dsimp [currentCtx']
+    rw [Sim.OpResultPtr.get!_BlockOperandPtr_removeFromCurrent]
+  case case2 =>
+    rename_i _ _ _ currentCtx currentIndex hCtxCur hOpCur hIndexCur currentCtx' hne ih
+    rw [ih]
+    dsimp [currentCtx']
+    rw [Sim.OpResultPtr.get!_BlockOperandPtr_removeFromCurrent]
+
+@[simp]
+theorem OpResultPtr.firstUse!_detachBlockOperands
+    (ctx : Sim.IRContext OpInfo) (operation : Sim.OperationPtr)
+    (result : Veir.OpResultPtr)
+    (hCtx : ctx.spec.FieldsInBounds) (hOp : operation.InBounds ctx)
+    (hCap : (operation.spec.get! ctx.spec).capBlockOperands =
+      operation.spec.getNumSuccessors! ctx.spec) :
+    (result.get! (Rewriter.detachBlockOperands ctx operation hCtx hOp hCap).spec).firstUse =
+      (result.get! ctx.spec).firstUse := by
+  simp only [Rewriter.detachBlockOperands_def, Rewriter.detachBlockOperandsSim]
+  split
+  · rfl
+  · apply OpResultPtr.firstUse!_detachBlockOperands_loop
+
+@[simp]
+theorem ValuePtr.getFirstUse!_detachOpIfAttached
+    (ctx : Sim.IRContext OpInfo) (operation : Sim.OperationPtr)
+    (value : Veir.ValuePtr) (hCtx : ctx.spec.FieldsInBounds)
+    (hOp : operation.InBounds ctx) :
+    value.getFirstUse! (Rewriter.detachOpIfAttached ctx operation hCtx hOp).spec =
+      value.getFirstUse! ctx.spec := by
+  simp only [Rewriter.detachOpIfAttached_def, Rewriter.detachOpIfAttachedSim]
+  split
+  · apply ValuePtr.getFirstUse!_detachOp
+  · rfl
+
+@[simp, grind =]
+theorem OperationPtr.getNumResults!_detachOpIfAttached
+    (ctx : Sim.IRContext OpInfo) (operation : Sim.OperationPtr)
+    (op' : Veir.OperationPtr) (hCtx : ctx.spec.FieldsInBounds)
+    (hOp : operation.InBounds ctx) :
+    op'.getNumResults! (Rewriter.detachOpIfAttached ctx operation hCtx hOp).spec =
+      op'.getNumResults! ctx.spec := by
+  simp only [Rewriter.detachOpIfAttached_def, Rewriter.detachOpIfAttachedSim]
+  split
+  · apply OperationPtr.getNumResults!_detachOp
+  · rfl
+
+@[simp, grind =]
+theorem OperationPtr.getNumResults!_detachOperands_loop
+    (ctx : Sim.IRContext OpInfo) (operation : Sim.OperationPtr)
+    (off : Int64) (index : UInt64) (op' : Veir.OperationPtr)
+    (hCtx : ctx.spec.FieldsInBounds) (hOp : operation.InBounds ctx)
+    (hIndex : index.toNat < operation.spec.getNumOperands! ctx.spec)
+    (hoff : off = Buffed.Operation.Offsets.operands operation.spec ctx.spec) :
+    op'.getNumResults! (Rewriter.detachOperands.loop ctx operation off index
+      hCtx hOp hIndex hoff).spec = op'.getNumResults! ctx.spec := by
+  simp only [Rewriter.detachOperands.loop_def]
+  fun_induction Rewriter.detachOperands.loopSim
+  case case1 =>
+    rename_i _ _ _ currentCtx hCtxCur hOpCur hIndexCur hoffCur currentCtx'
+    dsimp [currentCtx']
+    rw [Sim.OperationPtr.getNumResults!_OpOperandPtr_removeFromCurrent]
+  case case2 =>
+    rename_i _ _ _ currentCtx currentIndex hCtxCur hOpCur hIndexCur hoffCur currentCtx' hne ih
+    rw [ih]
+    dsimp [currentCtx']
+    rw [Sim.OperationPtr.getNumResults!_OpOperandPtr_removeFromCurrent]
+
+@[simp, grind =]
+theorem OperationPtr.getNumResults!_detachOperands
+    (ctx : Sim.IRContext OpInfo) (operation : Sim.OperationPtr)
+    (op' : Veir.OperationPtr) (hCtx : ctx.spec.FieldsInBounds)
+    (hOp : operation.InBounds ctx)
+    (hCap : (operation.spec.get! ctx.spec).capOperands =
+      operation.spec.getNumOperands! ctx.spec) :
+    op'.getNumResults! (Rewriter.detachOperands ctx operation hCtx hOp hCap).spec =
+      op'.getNumResults! ctx.spec := by
+  simp only [Rewriter.detachOperands_def, Rewriter.detachOperandsSim]
+  split
+  · rfl
+  · apply OperationPtr.getNumResults!_detachOperands_loop
+
+@[simp, grind =]
+theorem OperationPtr.getNumResults!_detachBlockOperands_loop
+    (ctx : Sim.IRContext OpInfo) (operation : Sim.OperationPtr)
+    (index : UInt64) (op' : Veir.OperationPtr)
+    (hCtx : ctx.spec.FieldsInBounds) (hOp : operation.InBounds ctx)
+    (hIndex : index.toNat < operation.spec.getNumSuccessors! ctx.spec) :
+    op'.getNumResults! (Rewriter.detachBlockOperands.loop ctx operation index
+      hCtx hOp hIndex).spec = op'.getNumResults! ctx.spec := by
+  simp only [Rewriter.detachBlockOperands.loop_def]
+  fun_induction Rewriter.detachBlockOperands.loopSim
+  case case1 =>
+    rename_i _ _ _ currentCtx hCtxCur hOpCur hIndexCur currentCtx'
+    dsimp [currentCtx']
+    rw [Sim.OperationPtr.getNumResults!_BlockOperandPtr_removeFromCurrent]
+  case case2 =>
+    rename_i _ _ _ currentCtx currentIndex hCtxCur hOpCur hIndexCur currentCtx' hne ih
+    rw [ih]
+    dsimp [currentCtx']
+    rw [Sim.OperationPtr.getNumResults!_BlockOperandPtr_removeFromCurrent]
+
+@[simp, grind =]
+theorem OperationPtr.getNumResults!_detachBlockOperands
+    (ctx : Sim.IRContext OpInfo) (operation : Sim.OperationPtr)
+    (op' : Veir.OperationPtr) (hCtx : ctx.spec.FieldsInBounds)
+    (hOp : operation.InBounds ctx)
+    (hCap : (operation.spec.get! ctx.spec).capBlockOperands =
+      operation.spec.getNumSuccessors! ctx.spec) :
+    op'.getNumResults! (Rewriter.detachBlockOperands ctx operation hCtx hOp hCap).spec =
+      op'.getNumResults! ctx.spec := by
+  simp only [Rewriter.detachBlockOperands_def, Rewriter.detachBlockOperandsSim]
+  split
+  · rfl
+  · apply OperationPtr.getNumResults!_detachBlockOperands_loop
+
+@[simp, grind =]
+theorem OperationPtr.getNumOperands!_detachOperands_loop
+    (ctx : Sim.IRContext OpInfo) (operation : Sim.OperationPtr)
+    (off : Int64) (index : UInt64) (op' : Veir.OperationPtr)
+    (hCtx : ctx.spec.FieldsInBounds) (hOp : operation.InBounds ctx)
+    (hIndex : index.toNat < operation.spec.getNumOperands! ctx.spec)
+    (hoff : off = Buffed.Operation.Offsets.operands operation.spec ctx.spec) :
+    op'.getNumOperands! (Rewriter.detachOperands.loop ctx operation off index
+      hCtx hOp hIndex hoff).spec = op'.getNumOperands! ctx.spec := by
+  simp only [Rewriter.detachOperands.loop_def]
+  fun_induction Rewriter.detachOperands.loopSim <;>
+    grind [Sim.OperationPtr.getNumOperands!_OpOperandPtr_removeFromCurrent]
+
+@[simp, grind =]
+theorem OperationPtr.getNumOperands!_detachOperands
+    (ctx : Sim.IRContext OpInfo) (operation : Sim.OperationPtr)
+    (op' : Veir.OperationPtr) (hCtx : ctx.spec.FieldsInBounds)
+    (hOp : operation.InBounds ctx)
+    (hCap : (operation.spec.get! ctx.spec).capOperands =
+      operation.spec.getNumOperands! ctx.spec) :
+    op'.getNumOperands! (Rewriter.detachOperands ctx operation hCtx hOp hCap).spec =
+      op'.getNumOperands! ctx.spec := by
+  simp only [Rewriter.detachOperands_def, Rewriter.detachOperandsSim]
+  split
+  · rfl
+  · apply OperationPtr.getNumOperands!_detachOperands_loop
+
+@[simp, grind =]
+theorem OperationPtr.getNumOperands!_detachBlockOperands_loop
+    (ctx : Sim.IRContext OpInfo) (operation : Sim.OperationPtr)
+    (index : UInt64) (op' : Veir.OperationPtr)
+    (hCtx : ctx.spec.FieldsInBounds) (hOp : operation.InBounds ctx)
+    (hIndex : index.toNat < operation.spec.getNumSuccessors! ctx.spec) :
+    op'.getNumOperands! (Rewriter.detachBlockOperands.loop ctx operation index
+      hCtx hOp hIndex).spec = op'.getNumOperands! ctx.spec := by
+  simp only [Rewriter.detachBlockOperands.loop_def]
+  fun_induction Rewriter.detachBlockOperands.loopSim <;>
+    grind [Sim.OperationPtr.getNumOperands!_BlockOperandPtr_removeFromCurrent]
+
+@[simp, grind =]
+theorem OperationPtr.getNumOperands!_detachBlockOperands
+    (ctx : Sim.IRContext OpInfo) (operation : Sim.OperationPtr)
+    (op' : Veir.OperationPtr) (hCtx : ctx.spec.FieldsInBounds)
+    (hOp : operation.InBounds ctx)
+    (hCap : (operation.spec.get! ctx.spec).capBlockOperands =
+      operation.spec.getNumSuccessors! ctx.spec) :
+    op'.getNumOperands! (Rewriter.detachBlockOperands ctx operation hCtx hOp hCap).spec =
+      op'.getNumOperands! ctx.spec := by
+  simp only [Rewriter.detachBlockOperands_def, Rewriter.detachBlockOperandsSim]
+  split
+  · rfl
+  · apply OperationPtr.getNumOperands!_detachBlockOperands_loop
+
+@[simp, grind =]
+theorem OperationPtr.getNumSuccessors!_detachBlockOperands_loop
+    (ctx : Sim.IRContext OpInfo) (operation : Sim.OperationPtr)
+    (index : UInt64) (op' : Veir.OperationPtr)
+    (hCtx : ctx.spec.FieldsInBounds) (hOp : operation.InBounds ctx)
+    (hIndex : index.toNat < operation.spec.getNumSuccessors! ctx.spec) :
+    op'.getNumSuccessors! (Rewriter.detachBlockOperands.loop ctx operation index
+      hCtx hOp hIndex).spec = op'.getNumSuccessors! ctx.spec := by
+  simp only [Rewriter.detachBlockOperands.loop_def]
+  fun_induction Rewriter.detachBlockOperands.loopSim <;>
+    grind [Sim.OperationPtr.getNumSuccessors!_BlockOperandPtr_removeFromCurrent]
+
+@[simp, grind =]
+theorem OperationPtr.getNumSuccessors!_detachBlockOperands
+    (ctx : Sim.IRContext OpInfo) (operation : Sim.OperationPtr)
+    (op' : Veir.OperationPtr) (hCtx : ctx.spec.FieldsInBounds)
+    (hOp : operation.InBounds ctx)
+    (hCap : (operation.spec.get! ctx.spec).capBlockOperands =
+      operation.spec.getNumSuccessors! ctx.spec) :
+    op'.getNumSuccessors! (Rewriter.detachBlockOperands ctx operation hCtx hOp hCap).spec =
+      op'.getNumSuccessors! ctx.spec := by
+  simp only [Rewriter.detachBlockOperands_def, Rewriter.detachBlockOperandsSim]
+  split
+  · rfl
+  · apply OperationPtr.getNumSuccessors!_detachBlockOperands_loop
+
+@[simp]
+theorem OperationPtr.parent!_detachOpIfAttached_self
+    (ctx : Sim.IRContext OpInfo) (operation : Sim.OperationPtr)
+    (hCtx : ctx.spec.FieldsInBounds) (hOp : operation.InBounds ctx) :
+    (operation.spec.get! (Rewriter.detachOpIfAttached ctx operation hCtx hOp).spec).parent =
+      none := by
+  simp only [Rewriter.detachOpIfAttached_def, Rewriter.detachOpIfAttachedSim]
+  split
+  · rw [OperationPtr.parent!_detachOp]
+    simp
+  · have hParentIB : (operation.getParent ctx hOp).InBounds ctx := by grind
+    have hParentSpec := Sim.OperationPtr.getParent_spec ctx operation hOp
+    grind [Sim.OptionBlockPtr.toOption_none_iff_spec_none,
+      OperationPtr.get!_eq_get]
+
+@[simp]
+theorem OperationPtr.parent!_detachOperands_loop
+    (ctx : Sim.IRContext OpInfo) (operation : Sim.OperationPtr)
+    (off : Int64) (index : UInt64) (op' : Veir.OperationPtr)
+    (hCtx : ctx.spec.FieldsInBounds) (hOp : operation.InBounds ctx)
+    (hIndex : index.toNat < operation.spec.getNumOperands! ctx.spec)
+    (hoff : off = Buffed.Operation.Offsets.operands operation.spec ctx.spec) :
+    (op'.get! (Rewriter.detachOperands.loop ctx operation off index
+      hCtx hOp hIndex hoff).spec).parent = (op'.get! ctx.spec).parent := by
+  simp only [Rewriter.detachOperands.loop_def]
+  fun_induction Rewriter.detachOperands.loopSim <;>
+    grind [Sim.OperationPtr.parent!_OpOperandPtr_removeFromCurrent]
+
+@[simp]
+theorem OperationPtr.parent!_detachOperands
+    (ctx : Sim.IRContext OpInfo) (operation : Sim.OperationPtr)
+    (op' : Veir.OperationPtr) (hCtx : ctx.spec.FieldsInBounds)
+    (hOp : operation.InBounds ctx)
+    (hCap : (operation.spec.get! ctx.spec).capOperands =
+      operation.spec.getNumOperands! ctx.spec) :
+    (op'.get! (Rewriter.detachOperands ctx operation hCtx hOp hCap).spec).parent =
+      (op'.get! ctx.spec).parent := by
+  simp only [Rewriter.detachOperands_def, Rewriter.detachOperandsSim]
+  split
+  · rfl
+  · apply OperationPtr.parent!_detachOperands_loop
+
+@[simp]
+theorem OperationPtr.parent!_detachBlockOperands_loop
+    (ctx : Sim.IRContext OpInfo) (operation : Sim.OperationPtr)
+    (index : UInt64) (op' : Veir.OperationPtr)
+    (hCtx : ctx.spec.FieldsInBounds) (hOp : operation.InBounds ctx)
+    (hIndex : index.toNat < operation.spec.getNumSuccessors! ctx.spec) :
+    (op'.get! (Rewriter.detachBlockOperands.loop ctx operation index
+      hCtx hOp hIndex).spec).parent = (op'.get! ctx.spec).parent := by
+  simp only [Rewriter.detachBlockOperands.loop_def]
+  fun_induction Rewriter.detachBlockOperands.loopSim <;>
+    grind [Sim.OperationPtr.parent!_BlockOperandPtr_removeFromCurrent]
+
+@[simp]
+theorem OperationPtr.parent!_detachBlockOperands
+    (ctx : Sim.IRContext OpInfo) (operation : Sim.OperationPtr)
+    (op' : Veir.OperationPtr) (hCtx : ctx.spec.FieldsInBounds)
+    (hOp : operation.InBounds ctx)
+    (hCap : (operation.spec.get! ctx.spec).capBlockOperands =
+      operation.spec.getNumSuccessors! ctx.spec) :
+    (op'.get! (Rewriter.detachBlockOperands ctx operation hCtx hOp hCap).spec).parent =
+      (op'.get! ctx.spec).parent := by
+  simp only [Rewriter.detachBlockOperands_def, Rewriter.detachBlockOperandsSim]
+  split
+  · rfl
+  · apply OperationPtr.parent!_detachBlockOperands_loop
+
+@[simp, grind =]
+theorem OperationPtr.getNumRegions!_detachOperands_loop
+    (ctx : Sim.IRContext OpInfo) (operation : Sim.OperationPtr)
+    (off : Int64) (index : UInt64) (op' : Veir.OperationPtr)
+    (hCtx : ctx.spec.FieldsInBounds) (hOp : operation.InBounds ctx)
+    (hIndex : index.toNat < operation.spec.getNumOperands! ctx.spec)
+    (hoff : off = Buffed.Operation.Offsets.operands operation.spec ctx.spec) :
+    op'.getNumRegions! (Rewriter.detachOperands.loop ctx operation off index
+      hCtx hOp hIndex hoff).spec = op'.getNumRegions! ctx.spec := by
+  simp only [Rewriter.detachOperands.loop_def]
+  fun_induction Rewriter.detachOperands.loopSim <;>
+    grind [Sim.OperationPtr.getNumRegions!_OpOperandPtr_removeFromCurrent]
+
+@[simp, grind =]
+theorem OperationPtr.getNumRegions!_detachOperands
+    (ctx : Sim.IRContext OpInfo) (operation : Sim.OperationPtr)
+    (op' : Veir.OperationPtr) (hCtx : ctx.spec.FieldsInBounds)
+    (hOp : operation.InBounds ctx)
+    (hCap : (operation.spec.get! ctx.spec).capOperands =
+      operation.spec.getNumOperands! ctx.spec) :
+    op'.getNumRegions! (Rewriter.detachOperands ctx operation hCtx hOp hCap).spec =
+      op'.getNumRegions! ctx.spec := by
+  simp only [Rewriter.detachOperands_def, Rewriter.detachOperandsSim]
+  split
+  · rfl
+  · apply OperationPtr.getNumRegions!_detachOperands_loop
+
+@[simp, grind =]
+theorem OperationPtr.getNumRegions!_detachBlockOperands_loop
+    (ctx : Sim.IRContext OpInfo) (operation : Sim.OperationPtr)
+    (index : UInt64) (op' : Veir.OperationPtr)
+    (hCtx : ctx.spec.FieldsInBounds) (hOp : operation.InBounds ctx)
+    (hIndex : index.toNat < operation.spec.getNumSuccessors! ctx.spec) :
+    op'.getNumRegions! (Rewriter.detachBlockOperands.loop ctx operation index
+      hCtx hOp hIndex).spec = op'.getNumRegions! ctx.spec := by
+  simp only [Rewriter.detachBlockOperands.loop_def]
+  fun_induction Rewriter.detachBlockOperands.loopSim <;>
+    grind [Sim.OperationPtr.getNumRegions!_BlockOperandPtr_removeFromCurrent]
+
+@[simp, grind =]
+theorem OperationPtr.getNumRegions!_detachBlockOperands
+    (ctx : Sim.IRContext OpInfo) (operation : Sim.OperationPtr)
+    (op' : Veir.OperationPtr) (hCtx : ctx.spec.FieldsInBounds)
+    (hOp : operation.InBounds ctx)
+    (hCap : (operation.spec.get! ctx.spec).capBlockOperands =
+      operation.spec.getNumSuccessors! ctx.spec) :
+    op'.getNumRegions! (Rewriter.detachBlockOperands ctx operation hCtx hOp hCap).spec =
+      op'.getNumRegions! ctx.spec := by
+  simp only [Rewriter.detachBlockOperands_def, Rewriter.detachBlockOperandsSim]
+  split
+  · rfl
+  · apply OperationPtr.getNumRegions!_detachBlockOperands_loop
+
+@[simp, grind =]
+theorem OperationPtr.getNumRegions!_detachOpIfAttached
+    (ctx : Sim.IRContext OpInfo) (operation : Sim.OperationPtr)
+    (op' : Veir.OperationPtr) (hCtx : ctx.spec.FieldsInBounds)
+    (hOp : operation.InBounds ctx) :
+    op'.getNumRegions! (Rewriter.detachOpIfAttached ctx operation hCtx hOp).spec =
+      op'.getNumRegions! ctx.spec := by
+  simp only [Rewriter.detachOpIfAttached_def, Rewriter.detachOpIfAttachedSim]
+  split
+  · apply OperationPtr.getNumRegions!_detachOp
+  · rfl
+
+theorem Rewriter.eraseOpDeallocatedSpec_wellFormed
+    (ctx : Sim.IRContext OpInfo) (op : Sim.OperationPtr)
+    (wf : ctx.spec.WellFormed)
+    (hCtx : ctx.spec.FieldsInBounds) (hOp : op.InBounds ctx)
+    (hOpers : (op.spec.get! ctx.spec).capOperands =
+      op.spec.getNumOperands! ctx.spec)
+    (hBlOpers : (op.spec.get! ctx.spec).capBlockOperands =
+      op.spec.getNumSuccessors! ctx.spec)
+    (noRegions : op.spec.getNumRegions! ctx.spec = 0)
+    (noUses : op.spec.hasUses! ctx.spec = false) :
+    let ctx₀ := Rewriter.detachOpIfAttached ctx op hCtx hOp
+    let ctx₁ := Rewriter.detachOperands ctx₀ op (by grind) (by grind [generic_ptr_grind])
+      (by grind)
+    let ctx₂ := Rewriter.detachBlockOperands ctx₁ op (by grind)
+      (by grind [generic_ptr_grind]) (by grind [detachOperands_def, detachOperandsSim])
+    ∀ hOpAfter : op.spec.InBounds ctx₂.spec,
+      (op.spec.dealloc ctx₂.spec hOpAfter).WellFormed := by
+  dsimp only
+  let ctx₀ := Rewriter.detachOpIfAttached ctx op hCtx hOp
+  have wf₀ : ctx₀.spec.WellFormed := by
+    exact Rewriter.detachOpIfAttached_WellFormed ctx wf hCtx op hOp
+  have hOp₀ : op.InBounds ctx₀ := by grind [generic_ptr_grind]
+  have hCap₀ : (op.spec.get! ctx₀.spec).capOperands =
+      op.spec.getNumOperands! ctx₀.spec := by
+    exact (wf₀.operations op.spec hOp₀.ib).capOperands_eq_numOperands
+  let ctx₁ := Rewriter.detachOperands ctx₀ op wf₀.inBounds hOp₀ hCap₀
+  have wf₁ : ctx₁.spec.WellFormed
+      ((∅ : Std.ExtHashSet OpOperandPtr).insertMany
+        ((0...op.spec.getNumOperands! ctx₀.spec).toList.map
+          (fun i => OpOperandPtr.mk op.spec i))) (∅ : Std.ExtHashSet BlockOperandPtr) := by
+    exact Rewriter.detachOperands_wellFormed ctx₀ op wf₀.inBounds hOp₀ hCap₀
+      wf₀ (by simp)
+  have hOp₁ : op.InBounds ctx₁ := by grind [generic_ptr_grind]
+  have hCap₁ : (op.spec.get! ctx₁.spec).capBlockOperands =
+      op.spec.getNumSuccessors! ctx₁.spec := by
+    exact (wf₁.operations op.spec hOp₁.ib).capBlockOperands_eq_numSuccessors
+  let ctx₂ := Rewriter.detachBlockOperands ctx₁ op wf₁.inBounds hOp₁ hCap₁
+  have wf₂ : ctx₂.spec.WellFormed
+      ((∅ : Std.ExtHashSet OpOperandPtr).insertMany
+        ((0...op.spec.getNumOperands! ctx₀.spec).toList.map
+          (fun i => OpOperandPtr.mk op.spec i)))
+      ((∅ : Std.ExtHashSet BlockOperandPtr).insertMany
+        ((0...op.spec.getNumSuccessors! ctx₁.spec).toList.map
+          (fun i => BlockOperandPtr.mk op.spec i))) := by
+    exact Rewriter.detachBlockOperands_wellFormed ctx₁ op wf₁.inBounds hOp₁ hCap₁
+      wf₁ (by simp)
+  have wfMissing : ctx₂.spec.WellFormed
+      (Std.ExtHashSet.fromOperands ctx₂.spec op.spec)
+      (Std.ExtHashSet.fromSuccessors ctx₂.spec op.spec) := by
+    apply cast (a := wf₂)
+    congr
+    · simp only [Std.ExtHashSet.fromOperands,
+        Std.ExtHashSet.insertMany_empty_eq_ofList, OperationPtr.getOpOperand_def]
+      congr 3
+      grind [detachOperands_def, detachOperandsSim]
+    · simp only [Std.ExtHashSet.fromSuccessors,
+        Std.ExtHashSet.insertMany_empty_eq_ofList, OperationPtr.getBlockOperand_def]
+      congr 3
+      grind [detachOperands_def, detachOperandsSim]
+  have hOp₂ : op.InBounds ctx₂ := by grind [generic_ptr_grind]
+  have hNoUses₂ : ¬ op.spec.hasUses ctx₂.spec := by
+    simp only [← OperationPtr.hasUses!_eq_hasUses (hin := hOp₂.ib), Bool.not_eq_true]
+    rw [OperationPtr.hasUses!_eq_false_iff_hasUses!_getResult_eq_false]
+    intro index hindex
+    simp only [ValuePtr.hasUses!_def, ValuePtr.getFirstUse!_opResult_eq,
+      Option.isSome_eq_false_iff, Option.isNone_iff_eq_none]
+    rw [OpResultPtr.firstUse!_detachBlockOperands]
+    apply OpResultPtr.firstUse!_detachOperands_eq_none_of_firstUse!_eq_none
+      (ctx := ctx₀) (operation := op) (result := op.spec.getResult index)
+      (hctx := wf₀) (hMissingUses := by simp)
+    · grind
+    · have hindex₀ : index < op.spec.getNumResults! ctx.spec := by
+        simpa only [ctx₂, OperationPtr.getNumResults!_detachBlockOperands,
+          ctx₁, OperationPtr.getNumResults!_detachOperands,
+          ctx₀, OperationPtr.getNumResults!_detachOpIfAttached] using hindex
+      have hNoUses :=
+        (OperationPtr.hasUses!_eq_false_iff_hasUses!_getResult_eq_false).mp
+          noUses index hindex₀
+      simp only [ValuePtr.hasUses!_def, ValuePtr.getFirstUse!_opResult_eq,
+        Option.isSome_eq_false_iff, Option.isNone_iff_eq_none] at hNoUses
+      change (ValuePtr.opResult (op.spec.getResult index)).getFirstUse! ctx₀.spec = none
+      exact (ValuePtr.getFirstUse!_detachOpIfAttached ctx op
+        (ValuePtr.opResult (op.spec.getResult index)) hCtx hOp).trans hNoUses
+  intro hOpAfter
+  apply IRContext.wellFormed_OperationPtr_dealloc wfMissing hNoUses₂
+  · simp only [ctx₂, OperationPtr.parent!_detachBlockOperands,
+      ctx₁, OperationPtr.parent!_detachOperands,
+      ctx₀, OperationPtr.parent!_detachOpIfAttached_self]
+  · simpa only [ctx₂, OperationPtr.getNumRegions!_detachBlockOperands,
+      ctx₁, OperationPtr.getNumRegions!_detachOperands,
+      ctx₀, OperationPtr.getNumRegions!_detachOpIfAttached] using noRegions
+
+@[grind .]
+theorem Rewriter.eraseOp_deallocFieldsInBounds
+    (ctx : Sim.IRContext OpInfo) (op : Sim.OperationPtr)
+    (wf : ctx.spec.WellFormed)
+    (noRegions : op.spec.getNumRegions! ctx.spec = 0)
+    (noUses : op.spec.hasUses! ctx.spec = false) :
+    Rewriter.EraseOpDeallocFieldsInBounds ctx op := by
+  intro hCtx hOp hOpers hBlOpers
+  dsimp only
+  intro hOpAfter
+  exact (Rewriter.eraseOpDeallocatedSpec_wellFormed ctx op wf hCtx hOp
+    hOpers hBlOpers noRegions noUses hOpAfter.ib).inBounds
+
+theorem Rewriter.eraseOp_WellFormed
+    (ctx : Sim.IRContext OpInfo) (op : Sim.OperationPtr)
+    (wf : ctx.spec.WellFormed)
+    (hCtx : ctx.spec.FieldsInBounds) (hOp : op.InBounds ctx)
+    (hOpers : (op.spec.get! ctx.spec).capOperands =
+      op.spec.getNumOperands! ctx.spec)
+    (hBlOpers : (op.spec.get! ctx.spec).capBlockOperands =
+      op.spec.getNumSuccessors! ctx.spec)
+    (noRegions : op.spec.getNumRegions! ctx.spec = 0)
+    (noUses : op.spec.hasUses! ctx.spec = false)
+    (hDealloc : Rewriter.EraseOpDeallocFieldsInBounds ctx op := by grind) :
+    (Rewriter.eraseOp ctx op hCtx hOp hOpers hBlOpers hDealloc).spec.WellFormed := by
+  simp only [Rewriter.eraseOp_def, Rewriter.eraseOpSim]
+  have hOpAfter : op.InBounds
+      (Rewriter.detachBlockOperands
+        (Rewriter.detachOperands (Rewriter.detachOpIfAttached ctx op hCtx hOp) op
+          (by grind) (by grind [generic_ptr_grind]) (by grind)) op
+        (by grind) (by grind [generic_ptr_grind])
+        (by grind [detachOperands_def, detachOperandsSim])) := by
+    apply (Sim.GenericPtr.iff_operation op).mp
+    rw [Rewriter.detachBlockOperands_inBounds]
+    rw [Rewriter.detachOperands_inBounds]
+    rw [Rewriter.detachOpIfAttached_inBounds]
+    exact (Sim.GenericPtr.iff_operation op).mpr hOp
+  exact Rewriter.eraseOpDeallocatedSpec_wellFormed ctx op wf hCtx hOp
+    hOpers hBlOpers noRegions noUses hOpAfter.ib
+
+end Veir
