Veir/Rewriter/WellFormed/InsertOp.lean
@@ -1,0 +1,38 @@
+module
+
+public import Veir.Rewriter.Basic
+public import Veir.Rewriter.LinkedList.WellFormed
+
+public section
+
+namespace Veir
+
+variable {OpInfo : Type} [HasOpInfo OpInfo] [SerializableOpInfo OpInfo]
+  [HasBuffedOpCode OpInfo]
+
+@[grind .]
+theorem Rewriter.insertOp?_WellFormed
+    (ctx : Sim.IRContext OpInfo) (newOp : Sim.OperationPtr) (ip : InsertPoint)
+    (newOpIn : newOp.InBounds ctx)
+    (ipIn : ip.InBounds ctx.spec)
+    (ctxIn : ctx.spec.FieldsInBounds)
+    (ipRepr : ip.IsRepr)
+    (wf : ctx.spec.WellFormed)
+    (heq : Rewriter.insertOp? ctx newOp ip newOpIn ipIn ctxIn ipRepr = some newCtx) :
+    newCtx.spec.WellFormed := by
+  simp only [Rewriter.insertOp?_def, Rewriter.insertOp?Sim] at heq
+  split at heq
+  · simp at heq
+  · rename_i parent hParent
+    have hParentIB : (ip.block ctx ipIn ipRepr).InBounds ctx :=
+      InsertPoint.block_InBounds ctxIn ipIn ipRepr ipIn
+    have hParentSpec : (ip.block ctx ipIn ipRepr).spec = some parent.spec :=
+      Sim.OptionBlockPtr.toOption_some hParentIB hParent
+    have hBlock : ip.block! ctx.spec = some parent.spec := by
+      rw [InsertPoint.block!_eq_block ip ctx ipIn ipRepr]
+      exact hParentSpec
+    apply Sim.IRContext.wellFormed_OperationPtr_linkBetweenWithParent wf heq
+      (ip := ip) <;>
+      grind [Option.maybe₁_def]
+
+end Veir
